bil_envScript.sml
@@ -13,44 +13,44 @@ open bil_auxiliaryTheory bil_immTheory bil_valuesTheory;
 
 val _ = new_theory "bil_env";
 
-val _ = Datatype `bil_var_t = Var string bil_type_t`;
+val _ = Datatype `bil_var_t = BVar string bil_type_t`;
 
-val bil_var_name_def = Define `bil_var_name (Var n _) = n`;
-val bil_var_type_def = Define `bil_var_type (Var _ ty) = ty`;
+val bil_var_name_def = Define `bil_var_name (BVar n _) = n`;
+val bil_var_type_def = Define `bil_var_type (BVar _ ty) = ty`;
 
 val _ = Datatype `bil_var_environment_t =
-    IrregularEnv
-  | RegularEnv (string |-> (bil_type_t # (bil_val_t option)))`;
+    BEnv_Irregular
+  | BEnv_Regular (string |-> (bil_type_t # (bil_val_t option)))`;
 
 
 (* Empty environment *)
-val empty_env_def = Define `empty_env = RegularEnv FEMPTY`
+val bil_empty_env_def = Define `bil_empty_env = BEnv_Regular FEMPTY`
 
-val is_env_regular_def = Define `
-  (is_env_regular IrregularEnv = F) /\
-  (is_env_regular (RegularEnv _) = T)`;
+val bil_is_regular_env_def = Define `
+  (bil_is_regular_env BEnv_Irregular = F) /\
+  (bil_is_regular_env (BEnv_Regular _) = T)`;
 
-val is_valid_env_def = Define `(is_valid_env IrregularEnv = F) /\
-  (is_valid_env (RegularEnv m) <=> FEVERY (\ (_, (ty, vo)).
+val bil_is_valid_env_def = Define `(bil_is_valid_env BEnv_Irregular = F) /\
+  (bil_is_valid_env (BEnv_Regular m) <=> FEVERY (\ (_, (ty, vo)).
      (case vo of NONE => T | SOME v => (SOME ty = type_of_bil_val v))) m)`;
 
-val is_valid_env_empty = store_thm ("is_valid_env_empty",
-  ``is_valid_env empty_env``,
-SIMP_TAC std_ss [is_valid_env_def, empty_env_def, finite_mapTheory.FEVERY_FEMPTY]);
+val bil_is_valid_env_empty = store_thm ("bil_is_valid_env_empty",
+  ``bil_is_valid_env bil_empty_env``,
+SIMP_TAC std_ss [bil_is_valid_env_def, bil_empty_env_def, finite_mapTheory.FEVERY_FEMPTY]);
 
-val is_env_regular_REWRS = store_thm ("is_env_regular_REWRS",
-``!env. is_env_regular env <=> (env <> IrregularEnv)``,
-Cases >> SIMP_TAC (srw_ss()) [is_env_regular_def]);
+val bil_is_regular_env_REWRS = store_thm ("bil_is_regular_env_REWRS",
+``!env. bil_is_regular_env env <=> (env <> BEnv_Irregular)``,
+Cases >> SIMP_TAC (srw_ss()) [bil_is_regular_env_def]);
 
 val bil_env_lookup_def = Define `
-  (bil_env_lookup varname IrregularEnv = NONE) /\
-  (bil_env_lookup varname (RegularEnv env) = FLOOKUP env varname)`;
+  (bil_env_lookup varname BEnv_Irregular = NONE) /\
+  (bil_env_lookup varname (BEnv_Regular env) = FLOOKUP env varname)`;
 
 val bil_env_update_def = Define `
-  (bil_env_update varname vo ty IrregularEnv = IrregularEnv) /\
-  (bil_env_update varname vo ty (RegularEnv env) =
-    if (?v. (vo = SOME v) /\ (SOME ty <> type_of_bil_val v)) then IrregularEnv else
-    (RegularEnv (env |+ (varname, (ty, vo)))))`;
+  (bil_env_update varname vo ty BEnv_Irregular = BEnv_Irregular) /\
+  (bil_env_update varname vo ty (BEnv_Regular env) =
+    if (?v. (vo = SOME v) /\ (SOME ty <> type_of_bil_val v)) then BEnv_Irregular else
+    (BEnv_Regular (env |+ (varname, (ty, vo)))))`;
 
 
 val bil_env_lookup_type_def = Define `
@@ -58,28 +58,28 @@ val bil_env_lookup_type_def = Define `
 
 val bil_env_check_type_def = Define `
   bil_env_check_type var env =
-    (bil_env_lookup_type (bil_var_name var) env = SOME (bil_var_type var))`
+    (bil_env_lookup_type (bil_var_name var) env = SOME (bil_var_type var))`;
 
 
 val bil_env_read_def = Define `bil_env_read v env =
   case (bil_env_lookup (bil_var_name v) env) of
-     NONE => Unknown
-   | SOME (_, NONE) => Unknown
-   | SOME (ty, SOME r) => if (ty = bil_var_type v) then r else Unknown`;
+     NONE => BVal_Unknown
+   | SOME (_, NONE) => BVal_Unknown
+   | SOME (ty, SOME r) => if (ty = bil_var_type v) then r else BVal_Unknown`;
 
 
 val bil_env_write_def = Define `bil_env_write v va env =
-  if (bil_env_check_type v env) then bil_env_update (bil_var_name v) (SOME va) (bil_var_type v) env else IrregularEnv`;
+  if (bil_env_check_type v env) then bil_env_update (bil_var_name v) (SOME va) (bil_var_type v) env else BEnv_Irregular`;
 
 
 val bil_env_write_Irregular = store_thm ("bil_env_write_Irregular",
-  ``!v va. (bil_env_write v va IrregularEnv) = IrregularEnv``,
+  ``!v va. (bil_env_write v va BEnv_Irregular) = BEnv_Irregular``,
 SIMP_TAC std_ss [bil_env_write_def, bil_env_update_def]);
 
 
 val bil_env_write_Irregular_WrongVal = store_thm ("bil_env_write_Irregular_WrongVal",
   ``!v va env. (type_of_bil_val va <> SOME (bil_var_type v)) ==>
-               (bil_env_write v va env = IrregularEnv)``,
+               (bil_env_write v va env = BEnv_Irregular)``,
 
 REPEAT GEN_TAC >>
 SIMP_TAC std_ss [bil_env_write_def, bil_env_check_type_def] >>
@@ -87,40 +87,41 @@ COND_CASES_TAC >> REWRITE_TAC[] >>
 Cases_on `env` >> SIMP_TAC std_ss [bil_env_update_def])
 
 
-val is_valid_env_lookup = store_thm ("is_valid_env_lookup",
-  ``!env vn ty v. is_valid_env env ==>
+val bil_is_valid_env_lookup = store_thm ("bil_is_valid_env_lookup",
+  ``!env vn ty v. bil_is_valid_env env ==>
                   (bil_env_lookup vn env = SOME (ty, SOME v)) ==>
                   (type_of_bil_val v = SOME ty)``,
 
-Cases >> SIMP_TAC std_ss [is_valid_env_def] >>
-rename1 `RegularEnv f` >>
+Cases >> SIMP_TAC std_ss [bil_is_valid_env_def] >>
+rename1 `BEnv_Regular f` >>
 SIMP_TAC (std_ss++QI_ss) [bil_env_lookup_def, finite_mapTheory.FEVERY_ALL_FLOOKUP] >>
 REPEAT STRIP_TAC >>
 Q.PAT_X_ASSUM `!k. _` (MP_TAC o Q.SPEC `vn`) >>
 ASM_SIMP_TAC std_ss []);
 
 
-val is_valid_env_read = store_thm ("is_valid_env_read",
-  ``!env v ty r. is_valid_env env ==>
+val bil_is_valid_env_read = store_thm ("bil_is_valid_env_read",
+  ``!env v ty r. bil_is_valid_env env ==>
                  (bil_env_read v env = r) ==>
-                 (r <> Unknown) ==>
+                 (r <> BVal_Unknown) ==>
                  (type_of_bil_val r = SOME (bil_var_type v))``,
 
 SIMP_TAC std_ss [bil_env_read_def] >>
 REPEAT GEN_TAC >>
 REPEAT CASE_TAC >> FULL_SIMP_TAC std_ss [type_of_bil_val_def, pairTheory.pair_case_thm] >>
-METIS_TAC[is_valid_env_lookup]);
+METIS_TAC[bil_is_valid_env_lookup]);
+
 
 val bil_env_read_EQ_Unknown = store_thm ("bil_env_read_EQ_Unknown",
-  ``!v env. is_valid_env env ==> (
-       (bil_env_read v env = Unknown) <=> (!r. (bil_env_lookup (bil_var_name v) env <> (SOME (bil_var_type v, SOME r)))))``,
+  ``!v env. bil_is_valid_env env ==> (
+       (bil_env_read v env = BVal_Unknown) <=> (!r. (bil_env_lookup (bil_var_name v) env <> (SOME (bil_var_type v, SOME r)))))``,
 
 REPEAT GEN_TAC >>
 SIMP_TAC std_ss [bil_env_read_def] >>
 REPEAT CASE_TAC >>
 STRIP_TAC >>
-rename1 `r = Unknown` >>
-`type_of_bil_val r = SOME (bil_var_type v)` by METIS_TAC[is_valid_env_lookup] >>
+rename1 `r = BVal_Unknown` >>
+`type_of_bil_val r = SOME (bil_var_type v)` by METIS_TAC[bil_is_valid_env_lookup] >>
 STRIP_TAC >>
 FULL_SIMP_TAC std_ss [type_of_bil_val_def]);
 
@@ -128,8 +129,8 @@ FULL_SIMP_TAC std_ss [type_of_bil_val_def]);
 
 
 val bil_env_varname_is_bound_def = Define `
-  (bil_env_varname_is_bound IrregularEnv var = F) /\
-  (bil_env_varname_is_bound (RegularEnv env) var = (var IN FDOM env))`;
+  (bil_env_varname_is_bound BEnv_Irregular var = F) /\
+  (bil_env_varname_is_bound (BEnv_Regular env) var = (var IN FDOM env))`;
 
 val bil_env_varname_is_bound_ALT_DEF = store_thm ("bil_env_varname_is_bound_ALT_DEF",
   ``!var env. bil_env_varname_is_bound env var <=> IS_SOME (bil_env_lookup_type var env)``,
@@ -147,11 +148,11 @@ SIMP_TAC std_ss [bil_env_varname_is_bound_ALT_DEF, bil_env_lookup_type_def,
 
 
 val bil_env_var_is_declared_def = Define `
-  (bil_env_var_is_declared env (Var vn ty) <=>
+  (bil_env_var_is_declared env (BVar vn ty) <=>
   (bil_env_lookup_type vn env = SOME ty))`;
 
 val bil_env_var_is_initialised_def = Define `
-  (bil_env_var_is_initialised env (Var vn ty) <=>
+  (bil_env_var_is_initialised env (BVar vn ty) <=>
   (?v. bil_env_lookup vn env = SOME (ty, SOME v)))`;
 
 
@@ -169,14 +170,14 @@ Cases >> SIMP_TAC std_ss [bil_env_var_is_declared_def,
 
 
 val _ = Datatype `bil_env_cond_t =
-  | EnvCond_varname_bound string
-  | EnvCond_var_declared bil_var_t
-  | EnvCond_var_initialised bil_var_t`;
+  | BEnvCond_varname_bound string
+  | BEnvCond_var_declared bil_var_t
+  | BEnvCond_var_initialised bil_var_t`;
 
 val bil_env_cond_eval_def = Define `
-  (bil_env_cond_eval env (EnvCond_varname_bound vn)  <=> bil_env_varname_is_bound   env vn) /\
-  (bil_env_cond_eval env (EnvCond_var_initialised v) <=> bil_env_var_is_initialised env v) /\
-  (bil_env_cond_eval env (EnvCond_var_declared v)    <=> bil_env_var_is_declared    env v)`;
+  (bil_env_cond_eval env (BEnvCond_varname_bound vn)  <=> bil_env_varname_is_bound   env vn) /\
+  (bil_env_cond_eval env (BEnvCond_var_initialised v) <=> bil_env_var_is_initialised env v) /\
+  (bil_env_cond_eval env (BEnvCond_var_declared v)    <=> bil_env_var_is_declared    env v)`;
 
 
 val bil_env_order_def = Define `
@@ -298,18 +299,18 @@ Cases_on `vo` >> (
 
 val bil_env_order_write = store_thm ("bil_env_order_write",
 ``!env v va.
-    is_env_regular (bil_env_write v va env) ==>
+    bil_is_regular_env (bil_env_write v va env) ==>
     bil_env_order env (bil_env_write v va env)``,
 
 SIMP_TAC std_ss [bil_env_write_def] >>
 REPEAT STRIP_TAC >>
-COND_CASES_TAC >> FULL_SIMP_TAC std_ss [is_env_regular_def] >>
+COND_CASES_TAC >> FULL_SIMP_TAC std_ss [bil_is_regular_env_def] >>
 Cases_on `env` >> (
   FULL_SIMP_TAC std_ss [bil_env_update_def, bil_env_order_REFL]
 ) >>
 FULL_SIMP_TAC std_ss [bil_env_check_type_def, bil_env_lookup_type_def] >>
 rename1 `SOME (FST xx)` >> Cases_on `xx` >> rename1 `FST (ty, vo)` >>
-Cases_on `SOME ty = type_of_bil_val va` >> FULL_SIMP_TAC std_ss [is_env_regular_def] >>
+Cases_on `SOME ty = type_of_bil_val va` >> FULL_SIMP_TAC std_ss [bil_is_regular_env_def] >>
 FULL_SIMP_TAC (std_ss++boolSimps.LIFT_COND_ss) [
     bil_env_order_def, bil_env_lookup_def,
     finite_mapTheory.FLOOKUP_UPDATE]
