bil_valuesScript.sml
@@ -19,18 +19,18 @@ val bil_imm_ss = rewrites ((type_rws ``:bil_imm_t``) @ (type_rws ``:bil_immtype_
 (* ------------------------------------------------------------------------- *)
 
 val _ = Datatype `bil_val_t =
-    Unknown
-  | Imm bil_imm_t
-  | Mem bil_immtype_t (*Addr-Type*) bil_immtype_t (* value-type *) (num -> num)
+    BVal_Unknown
+  | BVal_Imm bil_imm_t
+  | BVal_Mem bil_immtype_t (*Addr-Type*) bil_immtype_t (* value-type *) (num -> num)
 `;
 
 
 val _ = Datatype `bil_type_t =
-    ImmType bil_immtype_t
-  | MemType bil_immtype_t (* Addr-Type *) bil_immtype_t (* Value-Type *)
+    BType_Imm bil_immtype_t
+  | BType_Mem bil_immtype_t (* Addr-Type *) bil_immtype_t (* Value-Type *)
 `;
 
-val BoolType_def = Define `BoolType = ImmType Bit1`;
+val BoolType_def = Define `BoolType = BType_Imm Bit1`;
 
 
 val bil_val_ss = rewrites (type_rws ``:bil_val_t``);
@@ -41,11 +41,11 @@ val bil_type_ss = rewrites (type_rws ``:bil_type_t``);
 (*  Checkers for Values                                                      *)
 (* ------------------------------------------------------------------------- *)
 
-val bil_val_is_Unknown_def = Define `bil_val_is_Unknown v = (v = Unknown)`;
-val bil_val_is_Imm_def = Define `bil_val_is_Imm v = ?b. (v = Imm b)`;
-val bil_val_is_Imm_s_def = Define `bil_val_is_Imm_s s v = ?n. (v = Imm (n2bs n s))`;
+val bil_val_is_Unknown_def = Define `bil_val_is_Unknown v = (v = BVal_Unknown)`;
+val bil_val_is_Imm_def = Define `bil_val_is_Imm v = ?b. (v = BVal_Imm b)`;
+val bil_val_is_Imm_s_def = Define `bil_val_is_Imm_s s v = ?n. (v = BVal_Imm (n2bs n s))`;
 val bil_val_is_Bool_def = Define `bil_val_is_Bool = bil_val_is_Imm_s Bit1`;
-val bil_val_is_Mem_def = Define `bil_val_is_Mem v = ?at vt mmap. (v = Mem at vt mmap)`;
+val bil_val_is_Mem_def = Define `bil_val_is_Mem v = ?at vt mmap. (v = BVal_Mem at vt mmap)`;
 
 val bil_val_checker_DEFS = save_thm ("bil_val_checker_DEFS", LIST_CONJ [
   bil_val_is_Unknown_def, bil_val_is_Imm_def, bil_val_is_Imm_s_def,
@@ -54,7 +54,7 @@ val bil_val_checker_DEFS = save_thm ("bil_val_checker_DEFS", LIST_CONJ [
 
 val bil_val_is_Imm_s_ALT_DEF = store_thm ("bil_val_is_Imm_s_ALT_DEF",
 ``!s v. bil_val_is_Imm_s s v <=>
-  (?b. (v = Imm b) /\ (type_of_bil_imm b = s))``,
+  (?b. (v = BVal_Imm b) /\ (type_of_bil_imm b = s))``,
 
 Cases_on `v` >> (
   SIMP_TAC (std_ss ++ bil_val_ss) [bil_val_is_Imm_s_def,
@@ -63,25 +63,25 @@ Cases_on `v` >> (
 
 
 val bil_val_checker_REWRS = store_thm ("bil_val_checker_REWRS",
-  ``bil_val_is_Unknown Unknown /\
-    (!b. ~bil_val_is_Unknown (Imm b)) /\
-    (!at vt mmap. ~(bil_val_is_Unknown (Mem at vt mmap))) /\
+  ``bil_val_is_Unknown BVal_Unknown /\
+    (!b. ~bil_val_is_Unknown (BVal_Imm b)) /\
+    (!at vt mmap. ~(bil_val_is_Unknown (BVal_Mem at vt mmap))) /\
 
-    ~(bil_val_is_Imm Unknown) /\
-    (!b. bil_val_is_Imm (Imm b)) /\
-    (!at vt mmap. ~(bil_val_is_Imm (Mem at vt mmap))) /\
+    ~(bil_val_is_Imm BVal_Unknown) /\
+    (!b. bil_val_is_Imm (BVal_Imm b)) /\
+    (!at vt mmap. ~(bil_val_is_Imm (BVal_Mem at vt mmap))) /\
 
-    ~(bil_val_is_Mem Unknown) /\
-    (!b. ~(bil_val_is_Mem (Imm b))) /\
-    (!at vt mmap. (bil_val_is_Mem (Mem at vt mmap))) /\
+    ~(bil_val_is_Mem BVal_Unknown) /\
+    (!b. ~(bil_val_is_Mem (BVal_Imm b))) /\
+    (!at vt mmap. (bil_val_is_Mem (BVal_Mem at vt mmap))) /\
 
-    (!s. ~(bil_val_is_Imm_s s Unknown)) /\
-    (!s b. bil_val_is_Imm_s s (Imm b) <=> (type_of_bil_imm b = s)) /\
-    (!s at vt mmap. ~(bil_val_is_Imm_s s (Mem at vt mmap))) /\
+    (!s. ~(bil_val_is_Imm_s s BVal_Unknown)) /\
+    (!s b. bil_val_is_Imm_s s (BVal_Imm b) <=> (type_of_bil_imm b = s)) /\
+    (!s at vt mmap. ~(bil_val_is_Imm_s s (BVal_Mem at vt mmap))) /\
 
-    (~(bil_val_is_Bool Unknown)) /\
-    (!b. bil_val_is_Bool (Imm b) <=> (type_of_bil_imm b = Bit1)) /\
-    (!at vt mmap. ~(bil_val_is_Bool (Mem at vt mmap)))``,
+    (~(bil_val_is_Bool BVal_Unknown)) /\
+    (!b. bil_val_is_Bool (BVal_Imm b) <=> (type_of_bil_imm b = Bit1)) /\
+    (!at vt mmap. ~(bil_val_is_Bool (BVal_Mem at vt mmap)))``,
 
 
   REWRITE_TAC[bil_val_is_Imm_s_ALT_DEF, bil_val_is_Bool_def] >>
@@ -105,52 +105,54 @@ SIMP_TAC (std_ss++bil_val_ss) [bil_val_is_Imm_def, bil_val_is_Bool_def,
 (* ------------------------------------------------------------------------- *)
 
 val type_of_bil_val_def = Define `
-  (type_of_bil_val Unknown = NONE) /\
-  (type_of_bil_val (Imm imm) = SOME (ImmType (type_of_bil_imm imm))) /\
-  (type_of_bil_val (Mem at vt _) = SOME (MemType at vt))`;
+  (type_of_bil_val BVal_Unknown = NONE) /\
+  (type_of_bil_val (BVal_Imm imm) = SOME (BType_Imm (type_of_bil_imm imm))) /\
+  (type_of_bil_val (BVal_Mem at vt _) = SOME (BType_Mem at vt))`;
 
-val bil_type_is_ImmType_def = Define `bil_type_is_ImmType ty = (?s. ty = ImmType s)`;
-val bil_type_is_ImmType_s_def = Define `bil_type_is_ImmType_s s ty = (ty = ImmType s)`
-val bil_type_is_BoolType_def = Define `bil_type_is_BoolType ty = (ty = ImmType Bit1)`
-val bil_type_is_MemType_def = Define `bil_type_is_MemType ty = (?at vt. ty = MemType at vt)`;
+val bil_type_is_Imm_def = Define `bil_type_is_Imm ty = (?s. ty = BType_Imm s)`;
+val bil_type_is_Imm_s_def = Define `bil_type_is_Imm_s s ty = (ty = BType_Imm s)`
+val bil_type_is_Bool_def = Define `bil_type_is_Bool ty = (ty = BType_Imm Bit1)`
+val bil_type_is_Mem_def = Define `bil_type_is_Mem ty = (?at vt. ty = BType_Mem at vt)`;
 
 val bil_type_checker_DEFS = save_thm ("bil_type_checker_DEFS", LIST_CONJ [
-  bil_type_is_ImmType_def, bil_type_is_ImmType_s_def,
-  bil_type_is_BoolType_def, bil_type_is_MemType_def]);
+  bil_type_is_Imm_def, bil_type_is_Imm_s_def,
+  bil_type_is_Bool_def, bil_type_is_Mem_def]);
 
 
 val bil_type_checker_REWRS = store_thm ("bil_type_checker_REWRS", ``
-    (!b. bil_type_is_ImmType (ImmType b)) /\
-    (!at vt. ~(bil_type_is_ImmType (MemType at vt))) /\
+    (!b. bil_type_is_Imm (BType_Imm b)) /\
+    (!at vt. ~(bil_type_is_Imm (BType_Mem at vt))) /\
 
-    (!b. ~(bil_type_is_MemType (ImmType b))) /\
-    (!at vt. (bil_type_is_MemType (MemType at vt))) /\
+    (!b. ~(bil_type_is_Mem (BType_Imm b))) /\
+    (!at vt. (bil_type_is_Mem (BType_Mem at vt))) /\
 
-    (!s b. bil_type_is_ImmType_s s (ImmType b) <=> (b = s)) /\
-    (!s at vt. ~(bil_type_is_ImmType_s s (MemType at vt))) /\
+    (!s b. bil_type_is_Imm_s s (BType_Imm b) <=> (b = s)) /\
+    (!s at vt. ~(bil_type_is_Imm_s s (BType_Mem at vt))) /\
 
-    (!b. bil_type_is_BoolType (ImmType b) <=> (b = Bit1)) /\
-    (!at vt. ~(bil_type_is_BoolType (MemType at vt)))``,
+    (!b. bil_type_is_Bool BoolType <=> T) /\
 
-  SIMP_TAC (std_ss ++ bil_type_ss) [bil_type_checker_DEFS]);
+    (!b. bil_type_is_Bool (BType_Imm b) <=> (b = Bit1)) /\
+    (!at vt. ~(bil_type_is_Bool (BType_Mem at vt)))``,
 
-
-val bil_type_is_ImmType_s_IMPL = store_thm ("bil_type_is_ImmType_s_IMPL",
-  ``!s v. bil_type_is_ImmType_s s v ==> bil_type_is_ImmType v``,
-SIMP_TAC (std_ss++bil_type_ss) [bil_type_is_ImmType_def, bil_type_is_ImmType_s_def]);
+  SIMP_TAC (std_ss ++ bil_type_ss) [bil_type_checker_DEFS, BoolType_def]);
 
 
-val bil_type_is_BoolType_IMPL = store_thm ("bil_type_is_BoolType_IMPL",
-  ``!v. bil_type_is_BoolType v ==> bil_type_is_ImmType v``,
-SIMP_TAC (std_ss++bil_type_ss) [bil_type_is_ImmType_def, bil_type_is_BoolType_def]);
+val bil_type_is_Imm_s_IMPL = store_thm ("bil_type_is_Imm_s_IMPL",
+  ``!s v. bil_type_is_Imm_s s v ==> bil_type_is_Imm v``,
+SIMP_TAC (std_ss++bil_type_ss) [bil_type_is_Imm_def, bil_type_is_Imm_s_def]);
+
+
+val bil_type_is_Bool_IMPL = store_thm ("bil_type_is_Bool_IMPL",
+  ``!v. bil_type_is_Bool v ==> bil_type_is_Imm v``,
+SIMP_TAC (std_ss++bil_type_ss) [bil_type_is_Imm_def, bil_type_is_Bool_def]);
 
 
 val type_of_bil_val_EQ_ELIMS = store_thm ("type_of_bil_val_EQ_ELIMS",
-  ``(!v. (type_of_bil_val v = NONE) <=> (v = Unknown)) /\
-    (!v ty. (type_of_bil_val v = SOME (ImmType ty)) <=>
-            (?i. (type_of_bil_imm i = ty) /\ (v = Imm i))) /\
-    (!v aty vty. (type_of_bil_val v = SOME (MemType aty vty)) <=>
-            (?f. (v = Mem aty vty f)))``,
+  ``(!v. (type_of_bil_val v = NONE) <=> (v = BVal_Unknown)) /\
+    (!v ty. (type_of_bil_val v = SOME (BType_Imm ty)) <=>
+            (?i. (type_of_bil_imm i = ty) /\ (v = BVal_Imm i))) /\
+    (!v aty vty. (type_of_bil_val v = SOME (BType_Mem aty vty)) <=>
+            (?f. (v = BVal_Mem aty vty f)))``,
 REPEAT CONJ_TAC >> Cases >> (
   SIMP_TAC (std_ss++bil_val_ss++bil_type_ss) [type_of_bil_val_def]
 ));
