bil_expScript.sml
@@ -22,20 +22,20 @@ val bil_type_ss = rewrites ((type_rws ``:bil_type_t``));
 (* ------------------------------------------------------------------------- *)
 
 val _ = Datatype `bil_exp_t =
-    Const             bil_imm_t
-  | Den               bil_var_t
+    BExp_Const             bil_imm_t
+  | BExp_Den               bil_var_t
 
-  | Cast              bil_cast_t bil_exp_t bil_immtype_t
+  | BExp_Cast              bil_cast_t bil_exp_t bil_immtype_t
 
-  | UnaryExp          bil_unary_exp_t bil_exp_t
-  | BinExp            bil_bin_exp_t bil_exp_t bil_exp_t
-  | BinPred           bil_bin_pred_t bil_exp_t bil_exp_t
+  | BExp_UnaryExp          bil_unary_exp_t bil_exp_t
+  | BExp_BinExp            bil_bin_exp_t bil_exp_t bil_exp_t
+  | BExp_BinPred           bil_bin_pred_t bil_exp_t bil_exp_t
 
     (* For some reason if-then-else officially misses in BAP documentation *)
-  | IfThenElse        bil_exp_t bil_exp_t bil_exp_t
+  | BExp_IfThenElse        bil_exp_t bil_exp_t bil_exp_t
 
-  | Load              bil_exp_t bil_exp_t bil_endian_t bil_immtype_t
-  | Store             bil_exp_t bil_exp_t bil_endian_t bil_exp_t
+  | BExp_Load              bil_exp_t bil_exp_t bil_endian_t bil_immtype_t
+  | BExp_Store             bil_exp_t bil_exp_t bil_endian_t bil_exp_t
 `;
 
 
@@ -44,75 +44,75 @@ val _ = Datatype `bil_exp_t =
 (* ------------------------------------------------------------------------- *)
 
 val bil_eval_cast_def = Define `
-  (bil_eval_cast ct (Imm bi) ty = Imm (bil_gencast ct bi ty)) /\
-  (bil_eval_cast _ _ _ = Unknown)`;
+  (bil_eval_cast ct (BVal_Imm bi) ty = BVal_Imm (bil_gencast ct bi ty)) /\
+  (bil_eval_cast _ _ _ = BVal_Unknown)`;
 
 val bil_eval_unary_exp_def = Define `
-  (bil_eval_unary_exp et (Imm bi) = Imm (bil_unary_exp et bi)) /\
-  (bil_eval_unary_exp _ _ = Unknown)`;
+  (bil_eval_unary_exp et (BVal_Imm bi) = BVal_Imm (bil_unary_exp et bi)) /\
+  (bil_eval_unary_exp _ _ = BVal_Unknown)`;
 
 val bil_eval_bin_exp_def = Define `
-  (bil_eval_bin_exp et (Imm bi1) (Imm bi2) =
-     if (type_of_bil_imm bi1 <> type_of_bil_imm bi2) then Unknown else
-     Imm (bil_bin_exp et bi1 bi2)) /\
-  (bil_eval_bin_exp _ _ _ = Unknown)`;
+  (bil_eval_bin_exp et (BVal_Imm bi1) (BVal_Imm bi2) =
+     if (type_of_bil_imm bi1 <> type_of_bil_imm bi2) then BVal_Unknown else
+     BVal_Imm (bil_bin_exp et bi1 bi2)) /\
+  (bil_eval_bin_exp _ _ _ = BVal_Unknown)`;
 
 val bil_eval_bin_pred_def = Define `
-  (bil_eval_bin_pred pt (Imm bi1) (Imm bi2) =
-     if (type_of_bil_imm bi1 <> type_of_bil_imm bi2) then Unknown else
-     Imm (bool2b (bil_bin_pred pt bi1 bi2))) /\
-  (bil_eval_bin_pred _ _ _ = Unknown)`;
+  (bil_eval_bin_pred pt (BVal_Imm bi1) (BVal_Imm bi2) =
+     if (type_of_bil_imm bi1 <> type_of_bil_imm bi2) then BVal_Unknown else
+     BVal_Imm (bool2b (bil_bin_pred pt bi1 bi2))) /\
+  (bil_eval_bin_pred _ _ _ = BVal_Unknown)`;
 
 val bil_eval_ifthenelse_def = Define `
-  (bil_eval_ifthenelse (Imm (Imm1 cw)) e1 e2 =
+  (bil_eval_ifthenelse (BVal_Imm (Imm1 cw)) e1 e2 =
      if (cw = 1w) then e1 else e2) /\
-  (bil_eval_ifthenelse _ _ _ = Unknown)`;
+  (bil_eval_ifthenelse _ _ _ = BVal_Unknown)`;
 
 val bil_eval_load_def = Define `
-  (bil_eval_load (Mem ta tv mmap) (Imm a) en t =
+  (bil_eval_load (BVal_Mem ta tv mmap) (BVal_Imm a) en t =
      if ((type_of_bil_imm a) = ta) then
         (case (bil_load_from_mem tv t mmap en (b2n a)) of
-           NONE => Unknown
-         | SOME i => Imm i)
-     else Unknown) /\
-  (bil_eval_load _ _ _ _ = Unknown)`;
+           NONE => BVal_Unknown
+         | SOME i => BVal_Imm i)
+     else BVal_Unknown) /\
+  (bil_eval_load _ _ _ _ = BVal_Unknown)`;
 
 val bil_eval_store_def = Define `
-  (bil_eval_store (Mem ta tv mmap) (Imm a) en (Imm v) =
+  (bil_eval_store (BVal_Mem ta tv mmap) (BVal_Imm a) en (BVal_Imm v) =
      if ((type_of_bil_imm a) = ta) then
         (case (bil_store_in_mem tv v mmap en (b2n a)) of
-           NONE => Unknown
-         | SOME mmap' => Mem ta tv mmap')
-     else Unknown) /\
-  (bil_eval_store _ _ _ _ = Unknown)`;
+           NONE => BVal_Unknown
+         | SOME mmap' => BVal_Mem ta tv mmap')
+     else BVal_Unknown) /\
+  (bil_eval_store _ _ _ _ = BVal_Unknown)`;
 
 
 
 val bil_eval_exp_def = Define `
-  (bil_eval_exp (Const n) env = Imm n) /\
+  (bil_eval_exp (BExp_Const n) env = BVal_Imm n) /\
 
-  (bil_eval_exp (Den v) env = bil_env_read v env) /\
+  (bil_eval_exp (BExp_Den v) env = bil_env_read v env) /\
 
-  (bil_eval_exp (Cast ct e ty) env = (
+  (bil_eval_exp (BExp_Cast ct e ty) env = (
      bil_eval_cast ct (bil_eval_exp e env) ty)) /\
 
-  (bil_eval_exp (UnaryExp et e) env = (
+  (bil_eval_exp (BExp_UnaryExp et e) env = (
      bil_eval_unary_exp et (bil_eval_exp e env))) /\
 
-  (bil_eval_exp (BinExp et e1 e2) env = (
+  (bil_eval_exp (BExp_BinExp et e1 e2) env = (
      bil_eval_bin_exp et (bil_eval_exp e1 env) (bil_eval_exp e2 env))) /\
 
-  (bil_eval_exp (BinPred pt e1 e2) env = (
+  (bil_eval_exp (BExp_BinPred pt e1 e2) env = (
      bil_eval_bin_pred pt (bil_eval_exp e1 env) (bil_eval_exp e2 env))) /\
 
-  (bil_eval_exp (IfThenElse c et ef) env =
+  (bil_eval_exp (BExp_IfThenElse c et ef) env =
      bil_eval_ifthenelse (bil_eval_exp c env) (bil_eval_exp et env) (bil_eval_exp ef env)
   ) /\
 
-  (bil_eval_exp (Load mem_e a_e en ty) env =
+  (bil_eval_exp (BExp_Load mem_e a_e en ty) env =
      bil_eval_load (bil_eval_exp mem_e env) (bil_eval_exp a_e env) en ty) /\
 
-  (bil_eval_exp (Store mem_e a_e en v_e) env =
+  (bil_eval_exp (BExp_Store mem_e a_e en v_e) env =
      bil_eval_store (bil_eval_exp mem_e env) (bil_eval_exp a_e env) en (bil_eval_exp v_e env))
 `;
 
@@ -124,26 +124,26 @@ val bil_eval_exp_def = Define `
 (* ------------------------------------------------------------------------- *)
 
 val bil_eval_cast_REWRS = store_thm ("bil_eval_cast_REWRS",
-``(!ct bi ty. (bil_eval_cast ct (Imm bi) ty = Imm (bil_gencast ct bi ty))) /\
-  (!ct ty. bil_eval_cast ct Unknown ty = Unknown) /\
-  (!ct at vt mmap ty. bil_eval_cast ct (Mem at vt mmap) ty = Unknown)``,
+``(!ct bi ty. (bil_eval_cast ct (BVal_Imm bi) ty = BVal_Imm (bil_gencast ct bi ty))) /\
+  (!ct ty. bil_eval_cast ct BVal_Unknown ty = BVal_Unknown) /\
+  (!ct at vt mmap ty. bil_eval_cast ct (BVal_Mem at vt mmap) ty = BVal_Unknown)``,
 SIMP_TAC std_ss [bil_eval_cast_def]);
 
 val bil_eval_unary_exp_REWRS = store_thm ("bil_eval_unary_exp_REWRS",
- ``(!et bi. (bil_eval_unary_exp et (Imm bi) = Imm (bil_unary_exp et bi))) /\
-   (!et. bil_eval_unary_exp et Unknown = Unknown) /\
-   (!et at vt mmap. bil_eval_unary_exp et (Mem at vt mmap) = Unknown)``,
+ ``(!et bi. (bil_eval_unary_exp et (BVal_Imm bi) = BVal_Imm (bil_unary_exp et bi))) /\
+   (!et. bil_eval_unary_exp et BVal_Unknown = BVal_Unknown) /\
+   (!et at vt mmap. bil_eval_unary_exp et (BVal_Mem at vt mmap) = BVal_Unknown)``,
 SIMP_TAC std_ss [bil_eval_unary_exp_def]);
 
 
 val bil_eval_bin_exp_REWRS = store_thm ("bil_eval_bin_exp_REWRS",
-``(!et bi1 bi2. bil_eval_bin_exp et (Imm bi1) (Imm bi2) =
-     if (type_of_bil_imm bi1 <> type_of_bil_imm bi2) then Unknown else
-     Imm (bil_bin_exp et bi1 bi2)) /\
-  (!et v. bil_eval_bin_exp et Unknown v = Unknown) /\
-  (!et v. bil_eval_bin_exp et v Unknown = Unknown) /\
-  (!et at vt mmap v. bil_eval_bin_exp et (Mem at vt mmap) v = Unknown) /\
-  (!et at vt mmap v. bil_eval_bin_exp et v (Mem at vt mmap) = Unknown)``,
+``(!et bi1 bi2. bil_eval_bin_exp et (BVal_Imm bi1) (BVal_Imm bi2) =
+     if (type_of_bil_imm bi1 <> type_of_bil_imm bi2) then BVal_Unknown else
+     BVal_Imm (bil_bin_exp et bi1 bi2)) /\
+  (!et v. bil_eval_bin_exp et BVal_Unknown v = BVal_Unknown) /\
+  (!et v. bil_eval_bin_exp et v BVal_Unknown = BVal_Unknown) /\
+  (!et at vt mmap v. bil_eval_bin_exp et (BVal_Mem at vt mmap) v = BVal_Unknown) /\
+  (!et at vt mmap v. bil_eval_bin_exp et v (BVal_Mem at vt mmap) = BVal_Unknown)``,
 SIMP_TAC std_ss [bil_eval_bin_exp_def] >>
 CONJ_TAC >| [
   Cases_on `v` >> SIMP_TAC std_ss [bil_eval_bin_exp_def],
@@ -151,13 +151,13 @@ CONJ_TAC >| [
 ]);
 
 val bil_eval_bin_pred_REWRS = store_thm ("bil_eval_bin_pred_REWRS",
-``(!et bi1 bi2. bil_eval_bin_pred et (Imm bi1) (Imm bi2) =
-     if (type_of_bil_imm bi1 <> type_of_bil_imm bi2) then Unknown else
-     Imm (bool2b (bil_bin_pred et bi1 bi2))) /\
-  (!et v. bil_eval_bin_pred et Unknown v = Unknown) /\
-  (!et v. bil_eval_bin_pred et v Unknown = Unknown) /\
-  (!et at vt mmap v. bil_eval_bin_pred et (Mem at vt mmap) v = Unknown) /\
-  (!et at vt mmap v. bil_eval_bin_pred et v (Mem at vt mmap) = Unknown)``,
+``(!et bi1 bi2. bil_eval_bin_pred et (BVal_Imm bi1) (BVal_Imm bi2) =
+     if (type_of_bil_imm bi1 <> type_of_bil_imm bi2) then BVal_Unknown else
+     BVal_Imm (bool2b (bil_bin_pred et bi1 bi2))) /\
+  (!et v. bil_eval_bin_pred et BVal_Unknown v = BVal_Unknown) /\
+  (!et v. bil_eval_bin_pred et v BVal_Unknown = BVal_Unknown) /\
+  (!et at vt mmap v. bil_eval_bin_pred et (BVal_Mem at vt mmap) v = BVal_Unknown) /\
+  (!et at vt mmap v. bil_eval_bin_pred et v (BVal_Mem at vt mmap) = BVal_Unknown)``,
 SIMP_TAC std_ss [bil_eval_bin_pred_def] >>
 CONJ_TAC >| [
   Cases_on `v` >> SIMP_TAC std_ss [bil_eval_bin_pred_def],
@@ -166,31 +166,31 @@ CONJ_TAC >| [
 
 
 val bil_eval_ifthenelse_REWRS = store_thm ("bil_eval_ifthenelse_REWRS",
-``(!c e1 e2. bil_eval_ifthenelse (Imm c) e1 e2 =
+``(!c e1 e2. bil_eval_ifthenelse (BVal_Imm c) e1 e2 =
      if (type_of_bil_imm c = Bit1) then (
        if (c = Imm1 1w) then e1 else e2
-     ) else Unknown) /\
-  (!c e1 e2. bil_eval_ifthenelse Unknown e1 e2 = Unknown) /\
-  (!at vt mmap e1 e2. bil_eval_ifthenelse (Mem at vt mmap) e1 e2 = Unknown)``,
+     ) else BVal_Unknown) /\
+  (!c e1 e2. bil_eval_ifthenelse BVal_Unknown e1 e2 = BVal_Unknown) /\
+  (!at vt mmap e1 e2. bil_eval_ifthenelse (BVal_Mem at vt mmap) e1 e2 = BVal_Unknown)``,
 SIMP_TAC std_ss [bil_eval_ifthenelse_def] >>
 Cases_on `c` >> (
   SIMP_TAC (std_ss++bil_imm_ss) [type_of_bil_imm_def, bil_eval_ifthenelse_def]
 ));
 
 val bil_eval_ifthenelse_REWRS_Unknown = store_thm ("bil_eval_ifthenelse_REWRS_Unknown",
-``(!ec e1 e2. 
-     (type_of_bil_val ec <> SOME (ImmType Bit1)) ==>
-     (bil_eval_ifthenelse ec e1 e2 = Unknown))``,
+``(!ec e1 e2.
+     (type_of_bil_val ec <> SOME (BType_Imm Bit1)) ==>
+     (bil_eval_ifthenelse ec e1 e2 = BVal_Unknown))``,
 
 Cases_on `ec` >> (
-  SIMP_TAC (std_ss++bil_type_ss++bil_imm_ss) [type_of_bil_imm_def, type_of_bil_val_def, 
+  SIMP_TAC (std_ss++bil_type_ss++bil_imm_ss) [type_of_bil_imm_def, type_of_bil_val_def,
     bil_eval_ifthenelse_REWRS]
 ));
 
 val bil_eval_ifthenelse_TF_EQ = store_thm ("bil_eval_ifthenelse_TF_EQ",
 ``!c e.
      bil_eval_ifthenelse c e e =
-     if (bil_val_is_Bool c) then e else Unknown``,
+     if (bil_val_is_Bool c) then e else BVal_Unknown``,
 Cases_on `c` >> (
   SIMP_TAC (std_ss++bil_imm_ss++bil_type_ss) [type_of_bil_imm_def, bil_eval_ifthenelse_REWRS,
     bil_val_checker_REWRS]
@@ -198,23 +198,23 @@ Cases_on `c` >> (
 
 
 val bil_eval_load_Unknown_REWRS1 = prove (
-  ``(!mem en t. bil_eval_load mem Unknown en t = Unknown) /\
-    (!mem en t aty vty mmap. bil_eval_load mem (Mem aty vty mmap) en t = Unknown)``,
+  ``(!mem en t. bil_eval_load mem BVal_Unknown en t = BVal_Unknown) /\
+    (!mem en t aty vty mmap. bil_eval_load mem (BVal_Mem aty vty mmap) en t = BVal_Unknown)``,
 
 SIMP_TAC std_ss [bil_eval_load_def] >>
 REPEAT CONJ_TAC >>
 Cases_on `mem` >> SIMP_TAC std_ss [bil_eval_load_def]);
 
 val bil_eval_load_Unknown_REWRS2 = prove (
-  ``(!a en t. bil_eval_load Unknown a en t = Unknown) /\
-    (!a en t i. bil_eval_load (Imm i) a en t = Unknown)``,
+  ``(!a en t. bil_eval_load BVal_Unknown a en t = BVal_Unknown) /\
+    (!a en t i. bil_eval_load (BVal_Imm i) a en t = BVal_Unknown)``,
 
 SIMP_TAC std_ss [bil_eval_load_def]);
 
 val bil_eval_load_Unknown_REWRS3 = prove (
   ``!a en t i aty vty mmap.
       (type_of_bil_imm i <> aty) ==>
-      (bil_eval_load (Mem aty vty mmap) (Imm i) en t = Unknown)``,
+      (bil_eval_load (BVal_Mem aty vty mmap) (BVal_Imm i) en t = BVal_Unknown)``,
 
 SIMP_TAC std_ss [bil_eval_load_def]);
 
@@ -222,7 +222,7 @@ SIMP_TAC std_ss [bil_eval_load_def]);
 val bil_eval_load_Unknown_REWRS4 = prove (
   ``!a en t i aty vty mmap.
       (t <> vty) ==>
-      (bil_eval_load (Mem aty vty mmap) (Imm i) NoEndian t = Unknown)``,
+      (bil_eval_load (BVal_Mem aty vty mmap) (BVal_Imm i) BEnd_NoEndian t = BVal_Unknown)``,
 
 SIMP_TAC std_ss [bil_eval_load_def] >>
 REPEAT STRIP_TAC >>
@@ -232,7 +232,7 @@ ASM_SIMP_TAC std_ss [bil_load_from_mem_NO_ENDIAN]);
 val bil_eval_load_Unknown_REWRS5 = prove (
   ``!a en t i aty vty mmap en.
       (bil_number_of_mem_splits vty t = NONE) ==>
-      (bil_eval_load (Mem aty vty mmap) (Imm i) en t = Unknown)``,
+      (bil_eval_load (BVal_Mem aty vty mmap) (BVal_Imm i) en t = BVal_Unknown)``,
 
 SIMP_TAC std_ss [bil_eval_load_def] >>
 REPEAT STRIP_TAC >>
@@ -242,27 +242,28 @@ ASM_SIMP_TAC std_ss [bil_load_from_mem_def]);
 
 val bil_eval_load_Unknown_REWRS = save_thm ("bil_eval_load_Unknown_REWRS",
   REWRITE_RULE [GSYM CONJ_ASSOC] (
-  LIST_CONJ [bil_eval_load_Unknown_REWRS1, bil_eval_load_Unknown_REWRS2, bil_eval_load_Unknown_REWRS3,
-             bil_eval_load_Unknown_REWRS4, bil_eval_load_Unknown_REWRS5]));
+  LIST_CONJ [bil_eval_load_Unknown_REWRS1, bil_eval_load_Unknown_REWRS2,
+             bil_eval_load_Unknown_REWRS3, bil_eval_load_Unknown_REWRS4,
+             bil_eval_load_Unknown_REWRS5]));
 
 
 val bil_eval_load_SINGLE_REWR = store_thm ("bil_eval_load_SINGLE_REWR",
   ``!a en t i aty vty mmap en.
-      (bil_eval_load (Mem aty vty mmap) (Imm i) en vty) =
-      ((if (type_of_bil_imm i = aty) then (Imm (n2bs (mmap (b2n i)) vty))
-       else Unknown))``,
+      (bil_eval_load (BVal_Mem aty vty mmap) (BVal_Imm i) en vty) =
+      ((if (type_of_bil_imm i = aty) then (BVal_Imm (n2bs (mmap (b2n i)) vty))
+       else BVal_Unknown))``,
 
 SIMP_TAC arith_ss [bil_eval_load_def, bil_load_from_mem_SINGLE]);
 
 
 val bil_eval_load_BASIC_REWR = store_thm ("bil_eval_load_BASIC_REWR",
   ``!a en t i aty vty ty mmap en.
-      (bil_eval_load (Mem aty vty mmap) (Imm i) en ty) =
+      (bil_eval_load (BVal_Mem aty vty mmap) (BVal_Imm i) en ty) =
       (if type_of_bil_imm i = aty then
         case bil_load_from_mem vty ty mmap en (b2n i) of
-          NONE => Unknown
-        | SOME i => Imm i
-       else Unknown)``,
+          NONE => BVal_Unknown
+        | SOME i => BVal_Imm i
+       else BVal_Unknown)``,
 SIMP_TAC arith_ss [bil_eval_load_def]);
 
 
@@ -270,13 +271,13 @@ val bil_eval_load_FULL_REWRS = save_thm ("bil_eval_load_FULL_REWRS",
 let
   val thm_prune0 = prove (``(!ta a.
       (type_of_bil_imm a <> ta) ==>
-      (bil_eval_load (Mem ta tv mmap) (Imm a) en tr = Unknown)) /\
+      (bil_eval_load (BVal_Mem ta tv mmap) (BVal_Imm a) en tr = BVal_Unknown)) /\
       (!tr tv.
       (tr <> tv) ==> (bil_number_of_mem_splits tv tr <> NONE) ==>
-      (bil_eval_load (Mem ta tv mmap) (Imm i) NoEndian tr = Unknown)) /\
+      (bil_eval_load (BVal_Mem ta tv mmap) (BVal_Imm i) BEnd_NoEndian tr = BVal_Unknown)) /\
       (!tr tv.
       (bil_number_of_mem_splits tv tr = NONE) ==>
-      (bil_eval_load (Mem ta tv mmap) (Imm i) en tr = Unknown))``,
+      (bil_eval_load (BVal_Mem ta tv mmap) (BVal_Imm i) en tr = BVal_Unknown))``,
    SIMP_TAC std_ss [bil_eval_load_Unknown_REWRS])
 
   val thm_prune1 = SIMP_RULE (std_ss ++ bil_imm_ss ++ DatatypeSimps.expand_type_quants_ss [``:bil_immtype_t``, ``:bil_imm_t``]) [bil_number_of_mem_splits_REWRS, type_of_bil_imm_def] thm_prune0
@@ -299,24 +300,26 @@ let
 in thm4
 end);
 
+
+
 val bil_eval_store_Unknown_REWRS1 = prove (
-  ``(!mem en v. bil_eval_store mem Unknown en v = Unknown) /\
-    (!mem en v aty vty mmap. bil_eval_store mem (Mem aty vty mmap) en v = Unknown)``,
+  ``(!mem en v. bil_eval_store mem BVal_Unknown en v = BVal_Unknown) /\
+    (!mem en v aty vty mmap. bil_eval_store mem (BVal_Mem aty vty mmap) en v = BVal_Unknown)``,
 
 SIMP_TAC std_ss [bil_eval_store_def] >>
 REPEAT CONJ_TAC >>
 Cases_on `mem` >> SIMP_TAC std_ss [bil_eval_store_def]);
 
 val bil_eval_store_Unknown_REWRS2 = prove (
-  ``(!a en v. bil_eval_store Unknown a en v = Unknown) /\
-    (!a en v i. bil_eval_store (Imm i) a en v = Unknown)``,
+  ``(!a en v. bil_eval_store BVal_Unknown a en v = BVal_Unknown) /\
+    (!a en v i. bil_eval_store (BVal_Imm i) a en v = BVal_Unknown)``,
 
 SIMP_TAC std_ss [bil_eval_store_def]);
 
 
 val bil_eval_store_Unknown_REWRS3 = prove (
-  ``(!a en mem. bil_eval_store mem a en Unknown = Unknown) /\
-    (!a en mem ta tv mmap. bil_eval_store mem a en (Mem ta tv mmap) = Unknown)``,
+  ``(!a en mem. bil_eval_store mem a en BVal_Unknown = BVal_Unknown) /\
+    (!a en mem ta tv mmap. bil_eval_store mem a en (BVal_Mem ta tv mmap) = BVal_Unknown)``,
 
 REPEAT CONJ_TAC >>
 Cases_on `mem` >> Cases_on `a` >> SIMP_TAC std_ss [bil_eval_store_def]);
@@ -325,7 +328,7 @@ Cases_on `mem` >> Cases_on `a` >> SIMP_TAC std_ss [bil_eval_store_def]);
 val bil_eval_store_Unknown_REWRS4 = prove (
   ``!en v i aty vty mmap.
       (type_of_bil_imm i <> aty) ==>
-      (bil_eval_store (Mem aty vty mmap) (Imm i) en v = Unknown)``,
+      (bil_eval_store (BVal_Mem aty vty mmap) (BVal_Imm i) en v = BVal_Unknown)``,
 Cases_on `v` >>
 SIMP_TAC std_ss [bil_eval_store_def]);
 
@@ -333,7 +336,7 @@ SIMP_TAC std_ss [bil_eval_store_def]);
 val bil_eval_store_Unknown_REWRS5 = prove (
   ``!a en v aty vty mmap.
       (type_of_bil_imm v <> vty) ==>
-      (bil_eval_store (Mem aty vty mmap) a NoEndian (Imm v) = Unknown)``,
+      (bil_eval_store (BVal_Mem aty vty mmap) a BEnd_NoEndian (BVal_Imm v) = BVal_Unknown)``,
 
 Cases_on `a` >> SIMP_TAC std_ss [bil_eval_store_def] >>
 REPEAT STRIP_TAC >>
@@ -344,7 +347,7 @@ ASM_SIMP_TAC std_ss [bil_store_in_mem_NO_ENDIAN]);
 val bil_eval_store_Unknown_REWRS6 = prove (
   ``!a en v aty vty mmap en.
       (bil_number_of_mem_splits vty (type_of_bil_imm v) = NONE) ==>
-      (bil_eval_store (Mem aty vty mmap) a en (Imm v) = Unknown)``,
+      (bil_eval_store (BVal_Mem aty vty mmap) a en (BVal_Imm v) = BVal_Unknown)``,
 
 Cases_on `a` >> SIMP_TAC std_ss [bil_eval_store_def, LET_DEF] >>
 REPEAT STRIP_TAC >>
@@ -354,14 +357,15 @@ ASM_SIMP_TAC std_ss [bil_store_in_mem_def, LET_DEF]);
 
 val bil_eval_store_Unknown_REWRS = save_thm ("bil_eval_store_Unknown_REWRS",
   SIMP_RULE std_ss [GSYM CONJ_ASSOC] (
-  LIST_CONJ [bil_eval_store_Unknown_REWRS1, bil_eval_store_Unknown_REWRS2, bil_eval_store_Unknown_REWRS3,
-             bil_eval_store_Unknown_REWRS4, bil_eval_store_Unknown_REWRS5, bil_eval_store_Unknown_REWRS6]));
+  LIST_CONJ [bil_eval_store_Unknown_REWRS1, bil_eval_store_Unknown_REWRS2,
+             bil_eval_store_Unknown_REWRS3, bil_eval_store_Unknown_REWRS4,
+             bil_eval_store_Unknown_REWRS5, bil_eval_store_Unknown_REWRS6]));
 
 val bil_eval_store_SINGLE_REWR = store_thm ("bil_eval_store_SINGLE_REWR",
   ``!a en t i aty v vty mmap en.
       ((type_of_bil_imm i = aty) /\ (type_of_bil_imm v = vty)) ==>
-      (bil_eval_store (Mem aty vty mmap) (Imm i) en (Imm v) =
-      (Mem aty vty ((b2n i =+ b2n v) mmap)))``,
+      (bil_eval_store (BVal_Mem aty vty mmap) (BVal_Imm i) en (BVal_Imm v) =
+      (BVal_Mem aty vty ((b2n i =+ b2n v) mmap)))``,
 
 SIMP_TAC arith_ss [bil_eval_store_def, bil_store_in_mem_SINGLE]);
 
@@ -369,12 +373,12 @@ SIMP_TAC arith_ss [bil_eval_store_def, bil_store_in_mem_SINGLE]);
 
 val bil_eval_store_BASIC_REWR = store_thm ("bil_eval_store_BASIC_REWR",
   ``!a en t i aty v vty mmap en.
-      (bil_eval_store (Mem aty vty mmap) (Imm i) en (Imm v) =
+      (bil_eval_store (BVal_Mem aty vty mmap) (BVal_Imm i) en (BVal_Imm v) =
       (if type_of_bil_imm i = aty then
          case bil_store_in_mem vty v mmap en (b2n i) of
-           NONE => Unknown
-         | SOME mmap' => Mem aty vty mmap'
-       else Unknown))``,
+           NONE => BVal_Unknown
+         | SOME mmap' => BVal_Mem aty vty mmap'
+       else BVal_Unknown))``,
 
 SIMP_TAC arith_ss [bil_eval_store_def]);
 
@@ -383,13 +387,13 @@ val bil_eval_store_FULL_REWRS = save_thm ("bil_eval_store_FULL_REWRS",
 let
   val thm_prune0 = prove (``(!ta a.
       (type_of_bil_imm a <> ta) ==>
-      (bil_eval_store (Mem ta tv mmap) (Imm a) en v = Unknown)) /\
+      (bil_eval_store (BVal_Mem ta tv mmap) (BVal_Imm a) en v = BVal_Unknown)) /\
       (!i tv.
       (type_of_bil_imm i <> tv) ==> (bil_number_of_mem_splits tv (type_of_bil_imm i) <> NONE) ==>
-      (bil_eval_store (Mem ta tv mmap) a NoEndian (Imm i) = Unknown)) /\
+      (bil_eval_store (BVal_Mem ta tv mmap) a BEnd_NoEndian (BVal_Imm i) = BVal_Unknown)) /\
       (!i tv.
       (bil_number_of_mem_splits tv (type_of_bil_imm i) = NONE) ==>
-      (bil_eval_store (Mem ta tv mmap) a en (Imm i) = Unknown))``,
+      (bil_eval_store (BVal_Mem ta tv mmap) a en (BVal_Imm i) = BVal_Unknown))``,
    SIMP_TAC std_ss [bil_eval_store_Unknown_REWRS])
 
   val thm_prune1 = SIMP_RULE (std_ss ++ bil_imm_ss ++ DatatypeSimps.expand_type_quants_ss [``:bil_immtype_t``, ``:bil_imm_t``]) [bil_number_of_mem_splits_REWRS, type_of_bil_imm_def] thm_prune0
@@ -418,7 +422,7 @@ end);
 (* ------------------------------------------------------------------------- *)
 
 val bil_dest_bool_val_def = Define `
-  (bil_dest_bool_val (Imm (Imm1 w)) = SOME (w = 1w)) /\
+  (bil_dest_bool_val (BVal_Imm (Imm1 w)) = SOME (w = 1w)) /\
   (bil_dest_bool_val _ = NONE)`
 
 val bil_dest_bool_val_EQ_NONE = store_thm ("bil_dest_bool_val_EQ_NONE",
