bil_programScript.sml
@@ -21,40 +21,40 @@ val _ = new_theory "bil_program";
 (* ------------------------------------------------------------------------- *)
 
 val _ = Datatype `bil_label_t =
-    Label string
-  | Address bil_imm_t
+    BL_Label string
+  | BL_Address bil_imm_t
 `;
 
 val _ = Datatype `bil_stmt_t =
-  | Declare bil_var_t
-  | Assign  bil_var_t bil_exp_t
-  | Jmp     bil_label_t
-  | CJmp    bil_exp_t bil_label_t bil_label_t
-  | Halt    bil_exp_t
-  | Assert  bil_exp_t
-  | Assume  bil_exp_t
+  | BStmt_Declare bil_var_t
+  | BStmt_Assign  bil_var_t bil_exp_t
+  | BStmt_Jmp     bil_label_t
+  | BStmt_CJmp    bil_exp_t bil_label_t bil_label_t
+  | BStmt_Halt    bil_exp_t
+  | BStmt_Assert  bil_exp_t
+  | BStmt_Assume  bil_exp_t
 `;
 
-val _ = Datatype `bil_block_t = <| label:bil_label_t ; statements:bil_stmt_t list |>`;
+val _ = Datatype `bil_block_t = <| bb_label:bil_label_t ; bb_statements:bil_stmt_t list |>`;
 val _ = Datatype `bil_program_t = BilProgram (bil_block_t list)`;
-val _ = Datatype `bil_programcounter_t = <| label:bil_label_t; index:num |>`;
+val _ = Datatype `bil_programcounter_t = <| bpc_label:bil_label_t; bpc_index:num |>`;
 
 val bil_pc_ss = rewrites (type_rws ``:bil_programcounter_t``);
 
 val _ = Datatype `bil_termcode_t =
-    Running
-  | Halted bil_val_t
-  | ReachedEnd
-  | ReachedUnknownLabel bil_label_t
-  | Failed
-  | AssumptionViolated`
+    BTC_Running
+  | BTC_Halted bil_val_t
+  | BTC_ReachedEnd
+  | BTC_ReachedUnknownLabel bil_label_t
+  | BTC_Failed
+  | BTC_AssumptionViolated`
 
 val _ = Datatype `bil_state_t = <|
-  pc       : bil_programcounter_t;
-  environ  : bil_var_environment_t;
-  termcode : bil_termcode_t;
-  debug    : string list;
-  execs    : num
+  bst_pc       : bil_programcounter_t;
+  bst_environ  : bil_var_environment_t;
+  bst_termcode : bil_termcode_t;
+  bst_debug    : string list;
+  bst_execs    : num
 |>`;
 
 val bil_state_ss = rewrites (type_rws ``:bil_state_t``);
@@ -65,14 +65,14 @@ val bil_termcode_ss = rewrites (type_rws ``:bil_termcode_t``);
 (* Programs                                                                  *)
 (* ------------------------------------------------------------------------- *)
 
-val bil_block_stmts_count_def = Define `bil_block_stmts_count bl = LENGTH bl.statements`;
+val bil_block_stmts_count_def = Define `bil_block_stmts_count bl = LENGTH bl.bb_statements`;
 val bil_program_stmts_count_def = Define`bil_program_stmts_count (BilProgram p) = SUM (MAP bil_block_stmts_count p)`;
 
 val bil_labels_of_program_def = Define `bil_labels_of_program (BilProgram p) =
-  MAP (\bl. bl.label) p`;
+  MAP (\bl. bl.bb_label) p`;
 
 val bil_is_valid_labels_def = Define `bil_is_valid_labels p =
-  ALL_DISTINCT (bil_labels_of_program p) /\ ~(MEM (Label "") (bil_labels_of_program p))`;
+  ALL_DISTINCT (bil_labels_of_program p) /\ ~(MEM (BL_Label "") (bil_labels_of_program p))`;
 
 val bil_is_valid_program_def = Define `bil_is_valid_program p <=>
    (bil_is_valid_labels p /\ bil_program_stmts_count p > 0)`;
@@ -80,11 +80,11 @@ val bil_is_valid_program_def = Define `bil_is_valid_program p <=>
 
 val bil_is_valid_labels_blocks_EQ_EL = store_thm ("bil_is_valid_labels_blocks_EQ_EL",
   ``!p n1 n2. (bil_is_valid_labels (BilProgram p) /\ n1 < LENGTH p /\ n2 < LENGTH p /\
-                ((EL n1 p).label = (EL n2 p).label)) ==> (n1 = n2)``,
+                ((EL n1 p).bb_label = (EL n2 p).bb_label)) ==> (n1 = n2)``,
 
 SIMP_TAC list_ss [bil_is_valid_labels_def, bil_labels_of_program_def] >>
 REPEAT STRIP_TAC >>
-MP_TAC (Q.ISPEC `MAP (\bl. bl.label) (p:bil_block_t list)` listTheory.EL_ALL_DISTINCT_EL_EQ) >>
+MP_TAC (Q.ISPEC `MAP (\bl. bl.bb_label) (p:bil_block_t list)` listTheory.EL_ALL_DISTINCT_EL_EQ) >>
 ASM_SIMP_TAC list_ss [GSYM LEFT_EXISTS_IMP_THM] >>
 Q.EXISTS_TAC `n1` >> Q.EXISTS_TAC `n2` >>
 ASM_SIMP_TAC list_ss [listTheory.EL_MAP]);
@@ -92,34 +92,34 @@ ASM_SIMP_TAC list_ss [listTheory.EL_MAP]);
 
 val bil_is_valid_labels_blocks_EQ = store_thm ("bil_is_valid_labels_blocks_EQ",
   ``!p bl1 bl2. (bil_is_valid_labels (BilProgram p) /\ MEM bl1 p /\ MEM bl2 p /\
-                (bl1.label = bl2.label)) ==> (bl1 = bl2)``,
+                (bl1.bb_label = bl2.bb_label)) ==> (bl1 = bl2)``,
 
 METIS_TAC [listTheory.MEM_EL, bil_is_valid_labels_blocks_EQ_EL]);
 
 
 
 val bil_get_program_block_info_by_label_def = Define `bil_get_program_block_info_by_label
-  (BilProgram p) l = INDEX_FIND 0 (\(x:bil_block_t). x.label = l) p
+  (BilProgram p) l = INDEX_FIND 0 (\(x:bil_block_t). x.bb_label = l) p
 `;
 
 val bil_get_program_block_info_by_label_THM = store_thm ("bil_get_program_block_info_by_label_THM",
-  ``(!p l. ((bil_get_program_block_info_by_label (BilProgram p) l = NONE) <=> (!bl. MEM bl p ==> (bl.label <> l)))) /\
+  ``(!p l. ((bil_get_program_block_info_by_label (BilProgram p) l = NONE) <=> (!bl. MEM bl p ==> (bl.bb_label <> l)))) /\
 
     (!p l i bl.
           (bil_get_program_block_info_by_label (BilProgram p) l = SOME (i, bl)) <=>
-          ((((i:num) < LENGTH p) /\ (EL i p = bl) /\ (bl.label = l) /\
-             (!j'. j' < i ==> (EL j' p).label <> l))))``,
+          ((((i:num) < LENGTH p) /\ (EL i p = bl) /\ (bl.bb_label = l) /\
+             (!j'. j' < i ==> (EL j' p).bb_label <> l))))``,
 
 SIMP_TAC list_ss [bil_get_program_block_info_by_label_def, INDEX_FIND_EQ_NONE,
   listTheory.EVERY_MEM, INDEX_FIND_EQ_SOME_0]);
 
 
 val bil_get_program_block_info_by_label_valid_THM = store_thm ("bil_get_program_block_info_by_label_valid_THM",
-  ``(!p l. ((bil_get_program_block_info_by_label (BilProgram p) l = NONE) <=> (!bl. MEM bl p ==> (bl.label <> l)))) /\
+  ``(!p l. ((bil_get_program_block_info_by_label (BilProgram p) l = NONE) <=> (!bl. MEM bl p ==> (bl.bb_label <> l)))) /\
 
     (!p l i bl. bil_is_valid_labels (BilProgram p) ==>
           ((bil_get_program_block_info_by_label (BilProgram p) l = SOME (i, bl)) <=>
-           ((i:num) < LENGTH p) /\ (EL i p = bl) /\ (bl.label = l)))``,
+           ((i:num) < LENGTH p) /\ (EL i p = bl) /\ (bl.bb_label = l)))``,
 
 SIMP_TAC (list_ss++boolSimps.EQUIV_EXTRACT_ss) [bil_get_program_block_info_by_label_def,
   INDEX_FIND_EQ_NONE, listTheory.EVERY_MEM, INDEX_FIND_EQ_SOME_0] >>
@@ -155,17 +155,17 @@ Cases_on `bil_get_program_block_info_by_label (BilProgram p) l` >| [
 (* ------------------------------------------------------------------------- *)
 
 val bil_is_valid_pc_def = Define `bil_is_valid_pc p pc =
-   (?i bl. (bil_get_program_block_info_by_label p (pc.label) = SOME (i, bl)) /\
-           (pc.index < LENGTH bl.statements))`;
+   (?i bl. (bil_get_program_block_info_by_label p (pc.bpc_label) = SOME (i, bl)) /\
+           (pc.bpc_index < LENGTH bl.bb_statements))`;
 
 val bil_is_end_pc_def = Define `bil_is_end_pc (BilProgram p) pc =
-   (?i bl. (bil_get_program_block_info_by_label (BilProgram p) (pc.label) = SOME (i, bl)) /\
-           (pc.index = LENGTH bl.statements) /\
-      (!j. (i < j /\ j < LENGTH p) ==> (((EL j p).statements) = [])))`;
+   (?i bl. (bil_get_program_block_info_by_label (BilProgram p) (pc.bpc_label) = SOME (i, bl)) /\
+           (pc.bpc_index = LENGTH bl.bb_statements) /\
+      (!j. (i < j /\ j < LENGTH p) ==> (((EL j p).bb_statements) = [])))`;
 
 val bil_is_allowed_pc_def = Define `bil_is_allowed_pc p pc =
-   (?i bl. (bil_get_program_block_info_by_label p (pc.label) = SOME (i, bl)) /\
-           (pc.index <= LENGTH bl.statements))`;
+   (?i bl. (bil_get_program_block_info_by_label p (pc.bpc_label) = SOME (i, bl)) /\
+           (pc.bpc_index <= LENGTH bl.bb_statements))`;
 
 
 val bil_is_valid_pc_not_end = store_thm ("bil_is_valid_pc_not_end",
@@ -177,8 +177,8 @@ SIMP_TAC arith_ss [bil_is_valid_pc_def, bil_is_end_pc_def,
 
 val bil_is_valid_pc_of_valid_blocks = store_thm ("bil_is_valid_pc_of_valid_blocks",
   ``!p pc. bil_is_valid_labels (BilProgram p) ==>
-           (bil_is_valid_pc (BilProgram p) pc <=> (?bl. MEM bl p /\ (pc.label = bl.label) /\
-             (pc.index < LENGTH bl.statements)))``,
+           (bil_is_valid_pc (BilProgram p) pc <=> (?bl. MEM bl p /\ (pc.bpc_label = bl.bb_label) /\
+             (pc.bpc_index < LENGTH bl.bb_statements)))``,
 SIMP_TAC std_ss [bil_is_valid_pc_def, bil_get_program_block_info_by_label_valid_THM,
   listTheory.MEM_EL, GSYM LEFT_EXISTS_AND_THM] >>
 METIS_TAC[]);
@@ -186,34 +186,34 @@ METIS_TAC[]);
 
 
 val bil_get_program_block_info_by_label_valid_pc = store_thm ("bil_get_program_block_info_by_label_valid_pc",
-  ``!p pc. bil_is_valid_pc p pc ==> IS_SOME (bil_get_program_block_info_by_label p pc.label)``,
+  ``!p pc. bil_is_valid_pc p pc ==> IS_SOME (bil_get_program_block_info_by_label p pc.bpc_label)``,
 
 SIMP_TAC std_ss [bil_is_valid_pc_def, GSYM LEFT_FORALL_IMP_THM]);
 
 val bil_get_current_statement_def = Define `bil_get_current_statement p pc =
-  option_CASE (bil_get_program_block_info_by_label p pc.label) NONE
-     (\ (_, bl). if (pc.index < LENGTH bl.statements) then SOME (EL (pc.index) bl.statements) else NONE) `;
+  option_CASE (bil_get_program_block_info_by_label p pc.bpc_label) NONE
+     (\ (_, bl). if (pc.bpc_index < LENGTH bl.bb_statements) then SOME (EL (pc.bpc_index) bl.bb_statements) else NONE) `;
 
 
 val bil_get_current_statement_IS_SOME = store_thm ("bil_get_current_statement_IS_SOME",
   ``!p pc. IS_SOME (bil_get_current_statement p pc) <=> bil_is_valid_pc p pc``,
 
 REPEAT GEN_TAC >>
-Cases_on `bil_get_program_block_info_by_label p pc.label` >> (
+Cases_on `bil_get_program_block_info_by_label p pc.bpc_label` >> (
   ASM_SIMP_TAC std_ss [bil_get_current_statement_def, bil_is_valid_pc_def]
 ) >>
 SIMP_TAC (std_ss++QI_ss++pairSimps.gen_beta_ss++boolSimps.LIFT_COND_ss) []);
 
 
 val bil_pc_normalise_def = Define `
-  (bil_pc_normalise (BilProgram p) pc = case bil_get_program_block_info_by_label (BilProgram p) (pc.label) of
-        SOME (n, bl) => if (pc.index < LENGTH bl.statements)
+  (bil_pc_normalise (BilProgram p) pc = case bil_get_program_block_info_by_label (BilProgram p) (pc.bpc_label) of
+        SOME (n, bl) => if (pc.bpc_index < LENGTH bl.bb_statements)
           then SOME pc
           else (
-            let p' = FILTER (\bl. bl.statements <> []) (DROP (SUC n) p) in
+            let p' = FILTER (\bl. bl.bb_statements <> []) (DROP (SUC n) p) in
             case p' of
               | [] => NONE
-              | (bl'::_) => SOME <| label := bl'.label ; index := 0 |>
+              | (bl'::_) => SOME <| bpc_label := bl'.bb_label ; bpc_index := 0 |>
             )
       | _ => NONE
   )
@@ -221,24 +221,24 @@ val bil_pc_normalise_def = Define `
 
 
 val bil_pc_next_def = Define `
-  bil_pc_next p pc = bil_pc_normalise p (pc with index updated_by SUC)`;
+  bil_pc_next p pc = bil_pc_normalise p (pc with bpc_index updated_by SUC)`;
 
 
 val bil_pc_normalise_EQ_SOME = store_thm ("bil_pc_normalise_EQ_SOME",
-``!p pc i bl pc'. (bil_get_program_block_info_by_label (BilProgram p) (pc.label) = SOME (i, bl)) ==>
+``!p pc i bl pc'. (bil_get_program_block_info_by_label (BilProgram p) (pc.bpc_label) = SOME (i, bl)) ==>
              ((bil_pc_normalise (BilProgram p) pc = SOME pc') <=>
-                (if (pc.index < LENGTH bl.statements) then (pc' = pc) else
-                (?j. (i < j /\ j < LENGTH p /\ ((EL j p).statements <> []) /\
-                     (pc' = <| label := (EL j p).label; index := 0 |>) /\
-                     (!j'. (i < j' /\ j' < j) ==> (((EL j' p).statements) = []))))))``,
+                (if (pc.bpc_index < LENGTH bl.bb_statements) then (pc' = pc) else
+                (?j. (i < j /\ j < LENGTH p /\ ((EL j p).bb_statements <> []) /\
+                     (pc' = <| bpc_label := (EL j p).bb_label; bpc_index := 0 |>) /\
+                     (!j'. (i < j' /\ j' < j) ==> (((EL j' p).bb_statements) = []))))))``,
 
 SIMP_TAC std_ss [bil_pc_normalise_def, pairTheory.pair_case_thm] >>
 REPEAT STRIP_TAC >>
-Cases_on `pc.index < LENGTH bl.statements` >- (
+Cases_on `pc.bpc_index < LENGTH bl.bb_statements` >- (
   ASM_SIMP_TAC arith_ss [] >> METIS_TAC[]
 ) >>
 ASM_SIMP_TAC std_ss [LET_DEF] >>
-Cases_on `FILTER (\bl. bl.statements <> []) (DROP (SUC i) p)` >| [
+Cases_on `FILTER (\bl. bl.bb_statements <> []) (DROP (SUC i) p)` >| [
   ASM_SIMP_TAC list_ss [LET_DEF] >>
   CCONTR_TAC >>
   FULL_SIMP_TAC std_ss [] >>
@@ -247,7 +247,7 @@ Cases_on `FILTER (\bl. bl.statements <> []) (DROP (SUC i) p)` >| [
      Q.EXISTS_TAC `j - SUC i` >>
      ASM_SIMP_TAC arith_ss []
   ) >>
-  `~(MEM (EL j p) (FILTER (\bl. bl.statements <> []) (DROP (SUC i) p)))` by
+  `~(MEM (EL j p) (FILTER (\bl. bl.bb_statements <> []) (DROP (SUC i) p)))` by
     ASM_SIMP_TAC list_ss [] >>
   FULL_SIMP_TAC list_ss [listTheory.MEM_FILTER] >>
   FULL_SIMP_TAC std_ss [],
@@ -266,7 +266,7 @@ Cases_on `FILTER (\bl. bl.statements <> []) (DROP (SUC i) p)` >| [
   Induct_on `p2` >- ASM_SIMP_TAC list_ss [] >>
   CONV_TAC (RENAME_VARS_CONV ["bl1"]) >>
   REPEAT STRIP_TAC >>
-  Cases_on `(bl1.statements) <> []` >> FULL_SIMP_TAC list_ss [] >| [
+  Cases_on `(bl1.bb_statements) <> []` >> FULL_SIMP_TAC list_ss [] >| [
     REPEAT (BasicProvers.VAR_EQ_TAC) >>
     EQ_TAC >> REPEAT STRIP_TAC >> REPEAT BasicProvers.VAR_EQ_TAC >> ASM_SIMP_TAC list_ss [] >| [
       Q.EXISTS_TAC `SUC i` >>
@@ -306,17 +306,17 @@ Cases_on `FILTER (\bl. bl.statements <> []) (DROP (SUC i) p)` >| [
 
 
 val bil_pc_normalise_EQ_NONE = store_thm ("bil_pc_normalise_EQ_NONE",
-``!p pc i bl. (bil_get_program_block_info_by_label (BilProgram p) (pc.label) = SOME (i, bl)) ==>
+``!p pc i bl. (bil_get_program_block_info_by_label (BilProgram p) (pc.bpc_label) = SOME (i, bl)) ==>
              ((bil_pc_normalise (BilProgram p) pc = NONE) <=> (
-                (LENGTH bl.statements <= pc.index) /\
-                (!j. (i < j /\ j < LENGTH p) ==> (((EL j p).statements) = []))))``,
+                (LENGTH bl.bb_statements <= pc.bpc_index) /\
+                (!j. (i < j /\ j < LENGTH p) ==> (((EL j p).bb_statements) = []))))``,
 
 SIMP_TAC std_ss [bil_pc_normalise_def, pairTheory.pair_case_thm] >>
 REPEAT STRIP_TAC >>
-Cases_on `pc.index < LENGTH bl.statements` >> (
+Cases_on `pc.bpc_index < LENGTH bl.bb_statements` >> (
   ASM_SIMP_TAC arith_ss []
 ) >>
-Cases_on `FILTER (\bl. bl.statements <> []) (DROP (SUC i) p)` >| [
+Cases_on `FILTER (\bl. bl.bb_statements <> []) (DROP (SUC i) p)` >| [
   ASM_SIMP_TAC list_ss [LET_DEF] >>
   REPEAT STRIP_TAC >>
   `MEM (EL j p) (DROP (SUC i) p)` by (
@@ -324,7 +324,7 @@ Cases_on `FILTER (\bl. bl.statements <> []) (DROP (SUC i) p)` >| [
      Q.EXISTS_TAC `j - SUC i` >>
      ASM_SIMP_TAC arith_ss []
   ) >>
-  `~(MEM (EL j p) (FILTER (\bl. bl.statements <> []) (DROP (SUC i) p)))` by
+  `~(MEM (EL j p) (FILTER (\bl. bl.bb_statements <> []) (DROP (SUC i) p)))` by
     ASM_SIMP_TAC list_ss [] >>
   FULL_SIMP_TAC list_ss [listTheory.MEM_FILTER] >>
   FULL_SIMP_TAC std_ss [],
@@ -332,7 +332,7 @@ Cases_on `FILTER (\bl. bl.statements <> []) (DROP (SUC i) p)` >| [
 
   rename1 `FILTER _ _ = bl0::bls` >>
   ASM_SIMP_TAC list_ss [LET_DEF] >>
-  `MEM bl0 (FILTER (\bl. bl.statements <> []) (DROP (SUC i) p))` by
+  `MEM bl0 (FILTER (\bl. bl.bb_statements <> []) (DROP (SUC i) p))` by
     ASM_SIMP_TAC list_ss [] >>
   POP_ASSUM MP_TAC >>
   FULL_SIMP_TAC list_ss [listTheory.MEM_FILTER] >>
@@ -368,19 +368,19 @@ FULL_SIMP_TAC (arith_ss++boolSimps.EQUIV_EXTRACT_ss) [bil_is_end_pc_def]);
 
 
 val bil_is_allowed_pc_inc_valid = store_thm ("bil_is_allowed_pc_inc_valid",
-``!p pc. bil_is_valid_pc p pc ==> bil_is_allowed_pc p (pc with index updated_by SUC)``,
+``!p pc. bil_is_valid_pc p pc ==> bil_is_allowed_pc p (pc with bpc_index updated_by SUC)``,
 
 SIMP_TAC (arith_ss++bil_pc_ss) [bil_is_valid_pc_def, bil_is_allowed_pc_def, GSYM LEFT_FORALL_IMP_THM]);
 
 val bil_is_allowed_pc_jmp = store_thm ("bil_is_allowed_pc_jmp",
 ``!l p. MEM l (bil_labels_of_program p) ==>
-        bil_is_allowed_pc p <| label := l; index := 0 |>``,
+        bil_is_allowed_pc p <| bpc_label := l; bpc_index := 0 |>``,
 
 SIMP_TAC (std_ss++bil_pc_ss) [bil_is_allowed_pc_def, GSYM bil_get_program_block_info_by_label_MEM]);
 
 
 val bil_pc_normalise_valid = store_thm ("bil_pc_normalise_valid",
-``!p pc pc'. (bil_is_valid_labels p /\ (MEM pc.label (bil_labels_of_program p)) /\
+``!p pc pc'. (bil_is_valid_labels p /\ (MEM pc.bpc_label (bil_labels_of_program p)) /\
               (bil_pc_normalise p pc = SOME pc')) ==>
              (bil_is_valid_pc p pc')``,
 
@@ -390,12 +390,12 @@ SIMP_TAC list_ss [bil_labels_of_program_def, bil_pc_normalise_EQ_SOME,
 REPEAT STRIP_TAC >>
 FULL_SIMP_TAC std_ss [listTheory.MEM_EL] >>
 rename1 `bl = EL i p` >>
-`bil_get_program_block_info_by_label (BilProgram p) pc.label = SOME (i, bl)` by
+`bil_get_program_block_info_by_label (BilProgram p) pc.bpc_label = SOME (i, bl)` by
   METIS_TAC[bil_get_program_block_info_by_label_valid_THM] >>
 
 MP_TAC (Q.SPECL [`p`, `pc`, `i`, `bl`, `pc'`] bil_pc_normalise_EQ_SOME) >>
 FULL_SIMP_TAC std_ss [bil_is_valid_pc_def] >>
-Cases_on `pc.index < LENGTH (EL i p).statements` >| [
+Cases_on `pc.bpc_index < LENGTH (EL i p).bb_statements` >| [
   ASM_SIMP_TAC std_ss [] >> METIS_TAC[],
 
   ASM_SIMP_TAC (std_ss++bil_pc_ss) [bil_get_program_block_info_by_label_valid_THM,
@@ -403,7 +403,7 @@ Cases_on `pc.index < LENGTH (EL i p).statements` >| [
   REPEAT STRIP_TAC >>
   Q.EXISTS_TAC `j` >>
   ASM_SIMP_TAC arith_ss [] >>
-  Cases_on `(EL j p).statements` >> FULL_SIMP_TAC list_ss []
+  Cases_on `(EL j p).bb_statements` >> FULL_SIMP_TAC list_ss []
 ]);
 
 
@@ -413,7 +413,7 @@ val bil_pc_next_valid = store_thm ("bil_pc_next_valid",
 
 REPEAT STRIP_TAC >>
 MATCH_MP_TAC bil_pc_normalise_valid >>
-Q.EXISTS_TAC `pc with index updated_by SUC` >>
+Q.EXISTS_TAC `pc with bpc_index updated_by SUC` >>
 Cases_on `p` >>
 FULL_SIMP_TAC (std_ss++bil_pc_ss) [bil_pc_next_def, bil_is_valid_pc_def, bil_labels_of_program_def,
   listTheory.MEM_MAP] >>
@@ -421,24 +421,24 @@ METIS_TAC[listTheory.MEM_EL, bil_get_program_block_info_by_label_valid_THM]);
 
 
 val bil_pc_first_def = Define
-  `bil_pc_first (BilProgram p) = let bl = HD (FILTER (\bl. (bl.statements) <> []) p) in
-    (<| label := bl.label; index := 0 |>):bil_programcounter_t`;
+  `bil_pc_first (BilProgram p) = let bl = HD (FILTER (\bl. (bl.bb_statements) <> []) p) in
+    (<| bpc_label := bl.bb_label; bpc_index := 0 |>):bil_programcounter_t`;
 
 val bil_pc_last_def = Define
-  `bil_pc_last (BilProgram p) = let bl = LAST (FILTER (\bl. (bl.statements) <> []) p) in
-    (<| label := bl.label; index := LENGTH bl.statements - 1 |>):bil_programcounter_t`;
+  `bil_pc_last (BilProgram p) = let bl = LAST (FILTER (\bl. (bl.bb_statements) <> []) p) in
+    (<| bpc_label := bl.bb_label; bpc_index := LENGTH bl.bb_statements - 1 |>):bil_programcounter_t`;
 
 
 val bil_program_stmts_count_FILTER_NEQ_NIL = store_thm ("bil_program_stmts_count_FILTER_NEQ_NIL",
   ``!p. (bil_program_stmts_count (BilProgram p) > 0) ==>
-    (?bl0 bls. (FILTER (\bl. bl.statements <> []) p = bl0 :: bls) /\
-              EVERY (\bl. (bl.statements <> []) /\ MEM bl p) (bl0::bls))``,
+    (?bl0 bls. (FILTER (\bl. bl.bb_statements <> []) p = bl0 :: bls) /\
+              EVERY (\bl. (bl.bb_statements <> []) /\ MEM bl p) (bl0::bls))``,
 
 Induct_on `p` >> (
   FULL_SIMP_TAC list_ss [bil_program_stmts_count_def, bil_block_stmts_count_def]
 ) >>
 CONV_TAC (RENAME_VARS_CONV ["bl"]) >> GEN_TAC >>
-Cases_on `bl.statements` >| [
+Cases_on `bl.bb_statements` >| [
   SIMP_TAC list_ss [] >>
   REPEAT STRIP_TAC >>
   FULL_SIMP_TAC list_ss [listTheory.EVERY_MEM],
@@ -457,9 +457,9 @@ SIMP_TAC (std_ss++bil_pc_ss) [bil_is_valid_pc_of_valid_blocks, bil_is_valid_prog
 ASSUME_TAC (Q.SPEC `p` bil_program_stmts_count_FILTER_NEQ_NIL) >>
 REPEAT STRIP_TAC >>
 FULL_SIMP_TAC list_ss [] >>
-rename1 `bl0.statements <> []` >>
+rename1 `bl0.bb_statements <> []` >>
 Q.EXISTS_TAC `bl0` >>
-Cases_on `bl0.statements` >> FULL_SIMP_TAC list_ss []);
+Cases_on `bl0.bb_statements` >> FULL_SIMP_TAC list_ss []);
 
 
 val bil_pc_last_valid = store_thm ("bil_pc_last_valid",
@@ -480,7 +480,7 @@ FULL_SIMP_TAC list_ss [listTheory.EVERY_MEM]);
 
 
 val bil_is_valid_pc_label_OK = store_thm ("bil_is_valid_pc_label_OK",
-  ``!p pc. bil_is_valid_pc p pc ==> MEM pc.label (bil_labels_of_program p)``,
+  ``!p pc. bil_is_valid_pc p pc ==> MEM pc.bpc_label (bil_labels_of_program p)``,
 
 Cases_on `p` >> rename1 `BilProgram p` >>
 SIMP_TAC std_ss [bil_is_valid_pc_def, listTheory.MEM_MAP,
@@ -501,13 +501,13 @@ ASM_SIMP_TAC std_ss [bil_pc_next_def,
 Cases_on `p` >> rename1 `BilProgram p` >>
 ASM_SIMP_TAC (std_ss++bil_pc_ss) [bil_pc_last_def, LET_THM, bil_is_end_pc_def] >>
 
-`FILTER (\bl. bl.statements <> []) p <> []` by (
+`FILTER (\bl. bl.bb_statements <> []) p <> []` by (
   STRIP_TAC  >>
   FULL_SIMP_TAC std_ss [bil_is_valid_pc_def, bil_get_program_block_info_by_label_THM] >>
-  `MEM (EL i p) (FILTER (\bl. bl.statements <> []) p)` suffices_by ASM_SIMP_TAC list_ss [] >>
+  `MEM (EL i p) (FILTER (\bl. bl.bb_statements <> []) p)` suffices_by ASM_SIMP_TAC list_ss [] >>
   SIMP_TAC list_ss [listTheory.MEM_FILTER, listTheory.MEM_EL] >>
   REPEAT STRIP_TAC >| [
-    Cases_on `(EL i p).statements` >> FULL_SIMP_TAC list_ss [],
+    Cases_on `(EL i p).bb_statements` >> FULL_SIMP_TAC list_ss [],
     METIS_TAC[]
   ]
 ) >>
@@ -519,12 +519,12 @@ REV_FULL_SIMP_TAC std_ss [bil_get_program_block_info_by_label_valid_THM] >>
 EQ_TAC >> STRIP_TAC >| [
   `~(i < i')` by (
     STRIP_TAC >>
-    `bl.statements = []` by METIS_TAC[] >>
+    `bl.bb_statements = []` by METIS_TAC[] >>
     FULL_SIMP_TAC list_ss []
   ) >>
   `~(i' < i)` by (
     STRIP_TAC >>
-    `(EL i p).statements = []` by METIS_TAC[] >>
+    `(EL i p).bb_statements = []` by METIS_TAC[] >>
     FULL_SIMP_TAC list_ss []
   ) >>
   `i' = i` by DECIDE_TAC >>
@@ -534,7 +534,7 @@ EQ_TAC >> STRIP_TAC >| [
   `i' = i` by METIS_TAC [bil_is_valid_labels_blocks_EQ_EL] >>
   FULL_SIMP_TAC arith_ss [] >>
   REPEAT STRIP_TAC >>
-  `~(LENGTH (EL j p).statements > 0)` by METIS_TAC[] >>
+  `~(LENGTH (EL j p).bb_statements > 0)` by METIS_TAC[] >>
   ASM_SIMP_TAC arith_ss []
 ]);
 
@@ -564,13 +564,13 @@ EVAL_TAC);
 
 (* Statement to string (useful for debugging purposes) *)
 val bil_stmt_to_string_def = Define `bil_stmt_to_string stmt = case stmt of
-  | Declare (Var s _) => CONCAT ["Declaration of "; s]
-  | Assign (Var s _) _ => CONCAT ["Assignment of "; s]
-  | Jmp _ => "Jump"
-  | CJmp _ _ _ => "Conditional Jump"
-  | Halt _ => "Halt"
-  | Assert _ => "Assert"
-  | Assume _ => "Assume"
+  | BStmt_Declare (BVar s _) => CONCAT ["Declaration of "; s]
+  | BStmt_Assign (BVar s _) _ => CONCAT ["Assignment of "; s]
+  | BStmt_Jmp _ => "Jump"
+  | BStmt_CJmp _ _ _ => "Conditional Jump"
+  | BStmt_Halt _ => "Halt"
+  | BStmt_Assert _ => "Assert"
+  | BStmt_Assume _ => "Assume"
   | _ => "-- unsupported statement"
 `;
 
@@ -580,43 +580,43 @@ val bil_stmt_to_string_def = Define `bil_stmt_to_string stmt = case stmt of
 (* ------------------------------------------------------------------------- *)
 
 val bil_state_add_execs_def = Define `bil_state_add_execs st n =
-  st with execs updated_by ($+ n)`;
+  st with bst_execs updated_by ($+ n)`;
 
 val bil_state_is_terminated_def = Define `bil_state_is_terminated st =
-  (st.termcode <> Running)`;
+  (st.bst_termcode <> BTC_Running)`;
 
 val bil_state_is_terminated_IMP = store_thm ("bil_state_is_terminated_IMP",
-  ``(!st. (st.termcode = Running) ==> ~(bil_state_is_terminated st)) /\
-    (!st. (st.termcode <> Running) ==> (bil_state_is_terminated st))``, 
+  ``(!st. (st.bst_termcode = BTC_Running) ==> ~(bil_state_is_terminated st)) /\
+    (!st. (st.bst_termcode <> BTC_Running) ==> (bil_state_is_terminated st))``,
   SIMP_TAC std_ss [bil_state_is_terminated_def]);
 
 val bil_state_is_failed_def = Define `bil_state_is_failed st =
-  (st.termcode = Failed)`;
+  (st.bst_termcode = BTC_Failed)`;
 
 val bil_state_set_failed_def = Define `bil_state_set_failed st msg =
-  (st with termcode := Failed) with debug updated_by (\dbg. msg::dbg)`
+  (st with bst_termcode := BTC_Failed) with bst_debug updated_by (\dbg. msg::dbg)`;
 
 val bil_state_set_failed_is_failed = store_thm ("bil_state_set_failed_is_failed",
   ``!st msg. bil_state_is_failed (bil_state_set_failed st msg)``,
 SIMP_TAC (std_ss ++ bil_state_ss) [bil_state_set_failed_def, bil_state_is_failed_def]);
 
 val bil_state_normalise_pc_def = Define `bil_state_normalise_pc p (st:bil_state_t) =
-  case bil_pc_normalise p st.pc of
-    | SOME pc' => (st with pc := pc')
-    | NONE => (st with termcode := ReachedEnd)`;
+  case bil_pc_normalise p st.bst_pc of
+    | SOME pc' => (st with bst_pc := pc')
+    | NONE => (st with bst_termcode := BTC_ReachedEnd)`;
 
 val bil_state_incr_pc_def = Define `bil_state_incr_pc p (st:bil_state_t) =
-  bil_state_normalise_pc p (st with pc := (st.pc with index updated_by SUC))`
+  bil_state_normalise_pc p (st with bst_pc := (st.bst_pc with bpc_index updated_by SUC))`
 
 val bil_state_set_pc_def = Define `bil_state_set_pc p (st:bil_state_t) pc' =
-  bil_state_normalise_pc p (st with pc := pc')`;
+  bil_state_normalise_pc p (st with bst_pc := pc')`;
 
 val bil_state_init_def = Define `bil_state_init p = <|
-    pc       := bil_pc_first p
-  ; environ  := empty_env
-  ; termcode := Running
-  ; debug    := []
-  ; execs    := 0
+    bst_pc       := bil_pc_first p
+  ; bst_environ  := bil_empty_env
+  ; bst_termcode := BTC_Running
+  ; bst_debug    := []
+  ; bst_execs    := 0
 |>`;
 
 
@@ -627,70 +627,70 @@ val bil_state_init_def = Define `bil_state_init p = <|
 (* Execution of Jmp, CJmp, Halt, Assert, Assume doesn't change environment *)
 
 val bil_declare_initial_value_def = Define `
-  (bil_declare_initial_value (ImmType _) = NONE) /\
-  (bil_declare_initial_value (MemType at vt) = SOME (Mem at vt (K 0)))`;
+  (bil_declare_initial_value (BType_Imm _) = NONE) /\
+  (bil_declare_initial_value (BType_Mem at vt) = SOME (BVal_Mem at vt (K 0)))`;
 
 val bil_exec_stmt_declare_def = Define `bil_exec_stmt_declare p v ty (st : bil_state_t) =
    let env = (
       let vo = bil_declare_initial_value ty in
-      if bil_env_varname_is_bound st.environ v then IrregularEnv else
-      bil_env_update v vo ty st.environ) in
-    if (is_env_regular env) then
-       bil_state_incr_pc p (st with environ := env)
+      if bil_env_varname_is_bound st.bst_environ v then BEnv_Irregular else
+      bil_env_update v vo ty st.bst_environ) in
+    if (bil_is_regular_env env) then
+       bil_state_incr_pc p (st with bst_environ := env)
     else
        bil_state_set_failed st (CONCAT ["irregular environment after "; bil_stmt_to_string
-          (Declare (Var v ty))])`;
+          (BStmt_Declare (BVar v ty))])`;
 
 val bil_exec_stmt_assign_def = Define `bil_exec_stmt_assign p v ex (st : bil_state_t) =
-   let env = bil_env_write v (bil_eval_exp ex st.environ) st.environ in
-    if (is_env_regular env) then
-       bil_state_incr_pc p (st with environ := env)
+   let env = bil_env_write v (bil_eval_exp ex st.bst_environ) st.bst_environ in
+    if (bil_is_regular_env env) then
+       bil_state_incr_pc p (st with bst_environ := env)
     else
        bil_state_set_failed st (CONCAT ["irregular environment after "; bil_stmt_to_string
-          (Assign v ex)])`;
+          (BStmt_Assign v ex)])`;
 
 val bil_exec_stmt_halt_def = Define `bil_exec_stmt_halt ex (st : bil_state_t) =
-    (st with termcode := Halted (bil_eval_exp ex st.environ))`
+    (st with bst_termcode := BTC_Halted (bil_eval_exp ex st.bst_environ))`;
 
 val bil_exec_stmt_jmp_def = Define `bil_exec_stmt_jmp p l (st : bil_state_t) =
     if (MEM l (bil_labels_of_program p)) then
-      bil_state_set_pc p st <| label := l; index := 0 |>
-    else (st with termcode := (ReachedUnknownLabel l))`;
+      bil_state_set_pc p st <| bpc_label := l; bpc_index := 0 |>
+    else (st with bst_termcode := (BTC_ReachedUnknownLabel l))`;
 
 val bil_exec_stmt_cjmp_def = Define `bil_exec_stmt_cjmp p ex l1 l2 (st : bil_state_t) =
-  case (bil_dest_bool_val (bil_eval_exp ex st.environ)) of
+  case (bil_dest_bool_val (bil_eval_exp ex st.bst_environ)) of
     | SOME T => bil_exec_stmt_jmp p l1 st
     | SOME F => bil_exec_stmt_jmp p l2 st
     | NONE => bil_state_set_failed st "condition of cjmp failed to evaluate"`;
 
 val bil_exec_stmt_assert_def = Define `bil_exec_stmt_assert p ex (st : bil_state_t) =
-  case (bil_dest_bool_val (bil_eval_exp ex st.environ)) of
+  case (bil_dest_bool_val (bil_eval_exp ex st.bst_environ)) of
     | SOME T => bil_state_incr_pc p st
     | SOME F => bil_state_set_failed st "assertion failed"
     | NONE => bil_state_set_failed st "condition of assert failed to evaluate"`
 
 val bil_exec_stmt_assume_def = Define `bil_exec_stmt_assume p ex (st : bil_state_t) =
-  case (bil_dest_bool_val (bil_eval_exp ex st.environ)) of
+  case (bil_dest_bool_val (bil_eval_exp ex st.bst_environ)) of
     | SOME T => bil_state_incr_pc p st
-    | SOME F => (st with termcode := AssumptionViolated)
+    | SOME F => (st with bst_termcode := BTC_AssumptionViolated)
     | NONE => bil_state_set_failed st "condition of assume failed to evaluate"`;
 
 
 val bil_exec_stmt_def = Define `
-  (bil_exec_stmt p (Jmp l) st = bil_exec_stmt_jmp p l st) /\
-  (bil_exec_stmt p (CJmp e l1 l2) st = bil_exec_stmt_cjmp p e l1 l2 st) /\
-  (bil_exec_stmt p (Declare v) st = bil_exec_stmt_declare p (bil_var_name v) (bil_var_type v) st) /\
-  (bil_exec_stmt p (Assert ex) st = bil_exec_stmt_assert p ex st) /\
-  (bil_exec_stmt p (Assume ex) st = bil_exec_stmt_assume p ex st) /\
-  (bil_exec_stmt p (Assign v ex) st = bil_exec_stmt_assign p v ex st) /\
-  (bil_exec_stmt p (Halt ex) st = bil_exec_stmt_halt ex st)`;
+  (bil_exec_stmt p (BStmt_Jmp l) st = bil_exec_stmt_jmp p l st) /\
+  (bil_exec_stmt p (BStmt_CJmp e l1 l2) st = bil_exec_stmt_cjmp p e l1 l2 st) /\
+  (bil_exec_stmt p (BStmt_Declare v) st = bil_exec_stmt_declare p (bil_var_name v) (bil_var_type v) st) /\
+  (bil_exec_stmt p (BStmt_Assert ex) st = bil_exec_stmt_assert p ex st) /\
+  (bil_exec_stmt p (BStmt_Assume ex) st = bil_exec_stmt_assume p ex st) /\
+  (bil_exec_stmt p (BStmt_Assign v ex) st = bil_exec_stmt_assign p v ex st) /\
+  (bil_exec_stmt p (BStmt_Halt ex) st = bil_exec_stmt_halt ex st)`;
 
 
 val bil_exec_step_def = Define `bil_exec_step p state =
   if (bil_state_is_terminated state) then state else
-  case (bil_get_current_statement p state.pc) of
+  case (bil_get_current_statement p state.bst_pc) of
     | NONE => bil_state_set_failed state "invalid program_counter"
-    | SOME stm => (bil_exec_stmt p stm state) with execs updated_by SUC
+    | SOME stm => (bil_exec_stmt p stm state) with bst_execs updated_by SUC
 `;
 
 
@@ -699,18 +699,18 @@ val bil_exec_step_def = Define `bil_exec_step p state =
 (* ------------------------------------------------------------------------- *)
 
 val bil_is_valid_state_def = Define `bil_is_valid_state p st <=>
-  ((is_valid_env st.environ) /\ (if st.termcode = ReachedEnd then bil_is_end_pc p st.pc else
-      bil_is_valid_pc p st.pc))`;
+  ((bil_is_valid_env st.bst_environ) /\ (if st.bst_termcode = BTC_ReachedEnd then bil_is_end_pc p st.bst_pc else
+      bil_is_valid_pc p st.bst_pc))`;
 
 val bil_state_init_valid = store_thm ("bil_state_init_valid",
   ``!p. bil_is_valid_program p ==> bil_is_valid_state p (bil_state_init p)``,
 
 SIMP_TAC (std_ss++bil_state_ss++bil_termcode_ss) [bil_is_valid_state_def, bil_state_init_def,
-  bil_pc_first_valid, is_valid_env_empty]);
+  bil_pc_first_valid, bil_is_valid_env_empty]);
 
 
 val bil_is_valid_state_exec_ignore = store_thm ("bil_is_valid_state_exec_ignore",
-  ``!p st f. bil_is_valid_state p (st with execs updated_by f) =
+  ``!p st f. bil_is_valid_state p (st with bst_execs updated_by f) =
              bil_is_valid_state p st``,
 SIMP_TAC (std_ss++bil_state_ss) [bil_is_valid_state_def]);
 
@@ -720,18 +720,18 @@ val bil_exec_step_valid_THM = store_thm ("bil_exec_step_valid_THM",
           (if bil_state_is_terminated st then
              (bil_exec_step p st = st)
            else
-             (bil_is_valid_pc p st.pc) /\
-             (?stmt. (bil_get_current_statement p st.pc = SOME stmt) /\
-                     (bil_exec_step p st = (bil_exec_stmt p stmt st with execs updated_by SUC))))``,
+             (bil_is_valid_pc p st.bst_pc) /\
+             (?stmt. (bil_get_current_statement p st.bst_pc = SOME stmt) /\
+                     (bil_exec_step p st = (bil_exec_stmt p stmt st with bst_execs updated_by SUC))))``,
 
 REPEAT STRIP_TAC >>
 SIMP_TAC std_ss [bil_exec_step_def] >>
 Cases_on `bil_state_is_terminated st` >> ASM_SIMP_TAC (std_ss++boolSimps.CONJ_ss) [] >>
-`st.termcode <> ReachedEnd` by (
+`st.bst_termcode <> BTC_ReachedEnd` by (
   STRIP_TAC >> FULL_SIMP_TAC (std_ss++bil_termcode_ss) [bil_state_is_terminated_def]
 ) >>
-`?stm. bil_get_current_statement p st.pc = SOME stm` by (
-  `IS_SOME (bil_get_current_statement p st.pc)` suffices_by METIS_TAC[optionTheory.IS_SOME_EXISTS] >>
+`?stm. bil_get_current_statement p st.bst_pc = SOME stm` by (
+  `IS_SOME (bil_get_current_statement p st.bst_pc)` suffices_by METIS_TAC[optionTheory.IS_SOME_EXISTS] >>
   FULL_SIMP_TAC std_ss [bil_get_current_statement_IS_SOME,
      bil_is_valid_state_def]
 ) >>
@@ -739,77 +739,77 @@ FULL_SIMP_TAC std_ss [bil_is_valid_state_def]);
 
 
 val bil_is_valid_state_set_failed = store_thm ("bil_is_valid_state_set_failed",
-  ``!p st msg. bil_is_valid_state p st /\ bil_is_valid_pc p st.pc ==>
+  ``!p st msg. bil_is_valid_state p st /\ bil_is_valid_pc p st.bst_pc ==>
                bil_is_valid_state p (bil_state_set_failed st msg)``,
 SIMP_TAC (std_ss++bil_termcode_ss++bil_state_ss) [bil_is_valid_state_def, bil_state_set_failed_def]);
 
 
 val bil_is_valid_state_incr_pc = store_thm ("bil_is_valid_state_incr_pc",
-  ``!p st. bil_is_valid_program p /\ bil_is_valid_state p st /\ bil_is_valid_pc p st.pc ==>
+  ``!p st. bil_is_valid_program p /\ bil_is_valid_state p st /\ bil_is_valid_pc p st.bst_pc ==>
            bil_is_valid_state p (bil_state_incr_pc p st)``,
 SIMP_TAC (std_ss++bil_state_ss++boolSimps.CONJ_ss) [bil_state_incr_pc_def, bil_is_valid_state_def,
   bil_state_normalise_pc_def, bil_is_valid_pc_not_end
 ] >>
 REPEAT GEN_TAC >> STRIP_TAC >>
-Cases_on `bil_pc_normalise p (st.pc with index updated_by SUC)` >- (
+Cases_on `bil_pc_normalise p (st.bst_pc with bpc_index updated_by SUC)` >- (
   ASM_SIMP_TAC (std_ss++bil_state_ss) [GSYM bil_pc_normalise_EQ_NONE_is_end_pc,
     bil_is_allowed_pc_inc_valid]
 ) >>
 rename1 `_ = SOME pc'` >>
 ASM_SIMP_TAC (std_ss++bil_pc_ss++bil_state_ss) [] >>
 MATCH_MP_TAC bil_pc_normalise_valid >>
-Q.EXISTS_TAC `st.pc with index updated_by SUC` >>
+Q.EXISTS_TAC `st.bst_pc with bpc_index updated_by SUC` >>
 FULL_SIMP_TAC (std_ss++bil_pc_ss) [bil_is_valid_pc_label_OK,
    bil_is_valid_program_def]);
 
 
 
 val bil_exec_step_valid_state_invar_declare = prove (
-  ``!p st v. (bil_is_valid_program p /\ bil_is_valid_state p st /\ bil_is_valid_pc p st.pc) ==>
-             bil_is_valid_state p (bil_exec_stmt p (Declare v) st)``,
-Cases_on `v` >> rename1 `Var v ty` >>
+  ``!p st v. (bil_is_valid_program p /\ bil_is_valid_state p st /\ bil_is_valid_pc p st.bst_pc) ==>
+             bil_is_valid_state p (bil_exec_stmt p (BStmt_Declare v) st)``,
+Cases_on `v` >> rename1 `BVar v ty` >>
 SIMP_TAC (std_ss++boolSimps.LIFT_COND_ss) [bil_exec_stmt_def, bil_exec_stmt_declare_def, LET_THM,
-  bil_is_valid_state_set_failed, is_env_regular_def, bil_var_type_def, bil_var_name_def] >>
+  bil_is_valid_state_set_failed, bil_is_regular_env_def, bil_var_type_def, bil_var_name_def] >>
 REPEAT STRIP_TAC >>
 MATCH_MP_TAC bil_is_valid_state_incr_pc >>
 ASM_SIMP_TAC (std_ss++bil_state_ss) [] >>
 FULL_SIMP_TAC (std_ss++bil_state_ss) [bil_is_valid_state_def] >>
-Q.PAT_X_ASSUM `is_env_regular _` MP_TAC >>
-Cases_on `st.environ` >> SIMP_TAC std_ss [bil_env_update_def, is_env_regular_def] >>
-COND_CASES_TAC >- SIMP_TAC std_ss [is_env_regular_def] >>
-FULL_SIMP_TAC (std_ss) [is_env_regular_def, is_valid_env_def] >>
+Q.PAT_X_ASSUM `bil_is_regular_env _` MP_TAC >>
+Cases_on `st.bst_environ` >> SIMP_TAC std_ss [bil_env_update_def, bil_is_regular_env_def] >>
+COND_CASES_TAC >- SIMP_TAC std_ss [bil_is_regular_env_def] >>
+FULL_SIMP_TAC (std_ss) [bil_is_regular_env_def, bil_is_valid_env_def] >>
 ConseqConv.CONSEQ_REWRITE_TAC ([finite_mapTheory.FEVERY_STRENGTHEN_THM], [], []) >>
 Cases_on `bil_declare_initial_value ty` >> FULL_SIMP_TAC std_ss []);
 
 
 val bil_exec_step_valid_state_invar_assign = prove (
-  ``!p st v ex. (bil_is_valid_program p /\ bil_is_valid_state p st /\ bil_is_valid_pc p st.pc) ==>
-                 bil_is_valid_state p (bil_exec_stmt p (Assign v ex) st)``,
-Cases_on `v` >> rename1 `Var v ty` >>
+  ``!p st v ex. (bil_is_valid_program p /\ bil_is_valid_state p st /\ bil_is_valid_pc p st.bst_pc) ==>
+                 bil_is_valid_state p (bil_exec_stmt p (BStmt_Assign v ex) st)``,
+Cases_on `v` >> rename1 `BVar v ty` >>
 SIMP_TAC (std_ss++boolSimps.LIFT_COND_ss) [bil_exec_stmt_def, bil_exec_stmt_assign_def, LET_THM,
-  bil_is_valid_state_set_failed, is_env_regular_def] >>
+  bil_is_valid_state_set_failed, bil_is_regular_env_def] >>
 REPEAT STRIP_TAC >>
 MATCH_MP_TAC bil_is_valid_state_incr_pc >>
 ASM_SIMP_TAC (std_ss++bil_state_ss) [] >>
 FULL_SIMP_TAC (std_ss++bil_state_ss) [bil_is_valid_state_def] >>
-Q.PAT_X_ASSUM `is_env_regular _` MP_TAC >>
+Q.PAT_X_ASSUM `bil_is_regular_env _` MP_TAC >>
 SIMP_TAC std_ss [bil_env_write_def] >>
-COND_CASES_TAC >> SIMP_TAC std_ss [is_env_regular_def, bil_var_name_def, bil_var_type_def] >>
-Cases_on `st.environ` >> SIMP_TAC std_ss [bil_env_update_def, is_env_regular_def] >>
-COND_CASES_TAC >> SIMP_TAC std_ss [is_env_regular_def, is_valid_env_def] >>
+COND_CASES_TAC >> SIMP_TAC std_ss [bil_is_regular_env_def, bil_var_name_def, bil_var_type_def] >>
+Cases_on `st.bst_environ` >> SIMP_TAC std_ss [bil_env_update_def, bil_is_regular_env_def] >>
+COND_CASES_TAC >> SIMP_TAC std_ss [bil_is_regular_env_def, bil_is_valid_env_def] >>
 ConseqConv.CONSEQ_REWRITE_TAC ([finite_mapTheory.FEVERY_STRENGTHEN_THM], [], []) >>
-FULL_SIMP_TAC std_ss [is_valid_env_def]);
+FULL_SIMP_TAC std_ss [bil_is_valid_env_def]);
 
 
 val bil_exec_step_valid_state_invar_jmp' = prove (
-  ``!p st l. (bil_is_valid_program p /\ bil_is_valid_state p st /\ bil_is_valid_pc p st.pc) ==>
+  ``!p st l. (bil_is_valid_program p /\ bil_is_valid_state p st /\ bil_is_valid_pc p st.bst_pc) ==>
              bil_is_valid_state p (bil_exec_stmt_jmp p l st)``,
 SIMP_TAC std_ss [bil_exec_stmt_jmp_def] >>
 REPEAT STRIP_TAC >>
 COND_CASES_TAC >| [
   ASM_SIMP_TAC (std_ss++bil_state_ss) [bil_is_valid_state_def, bil_state_set_pc_def,
     bil_state_normalise_pc_def] >>
-  Cases_on `bil_pc_normalise p <|label := l; index := 0|>` >| [
+  Cases_on `bil_pc_normalise p <|bpc_label := l; bpc_index := 0|>` >| [
     FULL_SIMP_TAC (std_ss++bil_state_ss) [bil_is_valid_state_def] >>
     ASM_SIMP_TAC std_ss [GSYM bil_pc_normalise_EQ_NONE_is_end_pc,
       bil_is_allowed_pc_jmp],
@@ -818,7 +818,7 @@ COND_CASES_TAC >| [
     FULL_SIMP_TAC (std_ss++bil_pc_ss++bil_state_ss) [bil_is_valid_state_def,
       bil_is_valid_pc_not_end] >>
     MATCH_MP_TAC bil_pc_normalise_valid >>
-    Q.EXISTS_TAC `<|label := l; index := 0|>` >>
+    Q.EXISTS_TAC `<| bpc_label := l; bpc_index := 0|>` >>
     FULL_SIMP_TAC (std_ss++bil_pc_ss) [bil_is_valid_program_def]
   ],
 
@@ -826,18 +826,18 @@ COND_CASES_TAC >| [
 ]);
 
 val bil_exec_step_valid_state_invar_jmp = prove (
-  ``!p st l. (bil_is_valid_program p /\ bil_is_valid_state p st /\ bil_is_valid_pc p st.pc) ==>
-             bil_is_valid_state p (bil_exec_stmt p (Jmp l) st)``,
+  ``!p st l. (bil_is_valid_program p /\ bil_is_valid_state p st /\ bil_is_valid_pc p st.bst_pc) ==>
+             bil_is_valid_state p (bil_exec_stmt p (BStmt_Jmp l) st)``,
 SIMP_TAC std_ss [bil_exec_stmt_def, bil_exec_step_valid_state_invar_jmp']);
 
 
 val bil_exec_step_valid_state_invar_cjmp = prove (
   ``!p st ex l1 l2.
-       (bil_is_valid_program p /\ bil_is_valid_state p st /\ bil_is_valid_pc p st.pc) ==>
-       bil_is_valid_state p (bil_exec_stmt p (CJmp ex l1 l2) st)``,
+       (bil_is_valid_program p /\ bil_is_valid_state p st /\ bil_is_valid_pc p st.bst_pc) ==>
+       bil_is_valid_state p (bil_exec_stmt p (BStmt_CJmp ex l1 l2) st)``,
 SIMP_TAC std_ss [bil_exec_stmt_def, bil_exec_stmt_cjmp_def] >>
 REPEAT STRIP_TAC >>
-Cases_on `bil_dest_bool_val (bil_eval_exp ex st.environ)` >- (
+Cases_on `bil_dest_bool_val (bil_eval_exp ex st.bst_environ)` >- (
   ASM_SIMP_TAC std_ss [bil_is_valid_state_set_failed]
 ) >>
 rename1 `SOME c` >>
@@ -847,20 +847,20 @@ Cases_on `c` >> (
 
 
 val bil_exec_step_valid_state_invar_halt = prove (
-  ``!p st ex. (bil_is_valid_program p /\ bil_is_valid_state p st /\ bil_is_valid_pc p st.pc) ==>
-               bil_is_valid_state p (bil_exec_stmt p (Halt ex) st)``,
+  ``!p st ex. (bil_is_valid_program p /\ bil_is_valid_state p st /\ bil_is_valid_pc p st.bst_pc) ==>
+               bil_is_valid_state p (bil_exec_stmt p (BStmt_Halt ex) st)``,
 
 SIMP_TAC (std_ss++bil_state_ss++bil_termcode_ss) [bil_exec_stmt_def, bil_exec_stmt_halt_def,
   bil_is_valid_state_def]);
 
 
 val bil_exec_step_valid_state_invar_assert = prove (
-  ``!p st ex. (bil_is_valid_program p /\ bil_is_valid_state p st /\ bil_is_valid_pc p st.pc) ==>
-               bil_is_valid_state p (bil_exec_stmt p (Assert ex) st)``,
+  ``!p st ex. (bil_is_valid_program p /\ bil_is_valid_state p st /\ bil_is_valid_pc p st.bst_pc) ==>
+               bil_is_valid_state p (bil_exec_stmt p (BStmt_Assert ex) st)``,
 
 SIMP_TAC (std_ss++bil_state_ss++bil_termcode_ss) [bil_exec_stmt_def, bil_exec_stmt_assert_def] >>
 REPEAT GEN_TAC >> STRIP_TAC >>
-Cases_on `bil_dest_bool_val (bil_eval_exp ex st.environ)` >- (
+Cases_on `bil_dest_bool_val (bil_eval_exp ex st.bst_environ)` >- (
   ASM_SIMP_TAC std_ss [bil_is_valid_state_set_failed]
 ) >>
 rename1 `SOME c` >>
@@ -871,12 +871,12 @@ Cases_on `c` >| [
 
 
 val bil_exec_step_valid_state_invar_assume = prove (
-  ``!p st ex. (bil_is_valid_program p /\ bil_is_valid_state p st /\ bil_is_valid_pc p st.pc) ==>
-               bil_is_valid_state p (bil_exec_stmt p (Assume ex) st)``,
+  ``!p st ex. (bil_is_valid_program p /\ bil_is_valid_state p st /\ bil_is_valid_pc p st.bst_pc) ==>
+               bil_is_valid_state p (bil_exec_stmt p (BStmt_Assume ex) st)``,
 
 SIMP_TAC (std_ss++bil_state_ss++bil_termcode_ss) [bil_exec_stmt_def, bil_exec_stmt_assume_def] >>
 REPEAT GEN_TAC >> STRIP_TAC >>
-Cases_on `bil_dest_bool_val (bil_eval_exp ex st.environ)` >- (
+Cases_on `bil_dest_bool_val (bil_eval_exp ex st.bst_environ)` >- (
   ASM_SIMP_TAC std_ss [bil_is_valid_state_set_failed]
 ) >>
 rename1 `SOME c` >>
@@ -921,26 +921,26 @@ Induct_on `n` >> (
 (* ------------------------------------------------------------------------- *)
 
 val bil_state_normalise_pc_execs = store_thm ("bil_state_normalise_pc_execs",
-  ``!p st. (bil_state_normalise_pc p st).execs = st.execs``,
+  ``!p st. (bil_state_normalise_pc p st).bst_execs = st.bst_execs``,
 REPEAT GEN_TAC >>
 SIMP_TAC std_ss [bil_state_normalise_pc_def] >>
-Cases_on `bil_pc_normalise p st.pc` >> (
+Cases_on `bil_pc_normalise p st.bst_pc` >> (
   ASM_SIMP_TAC (std_ss++bil_state_ss) []
 ));
 
 
 val bil_state_incr_pc_execs = store_thm ("bil_state_incr_pc_execs",
-  ``!p st. (bil_state_incr_pc p st).execs = st.execs``,
+  ``!p st. (bil_state_incr_pc p st).bst_execs = st.bst_execs``,
 SIMP_TAC (std_ss++bil_state_ss) [bil_state_incr_pc_def, bil_state_normalise_pc_execs]);
 
 
 val bil_state_set_failed_execs = store_thm ("bil_state_set_failed_execs",
-  ``!st msg. (bil_state_set_failed st msg).execs = st.execs``,
+  ``!st msg. (bil_state_set_failed st msg).bst_execs = st.bst_execs``,
 SIMP_TAC (std_ss++bil_state_ss) [bil_state_set_failed_def]);
 
 
 val bil_state_set_pc_execs = store_thm ("bil_state_set_pc_execs",
-  ``!st p pc'. (bil_state_set_pc p st pc').execs = st.execs``,
+  ``!st p pc'. (bil_state_set_pc p st pc').bst_execs = st.bst_execs``,
 SIMP_TAC (std_ss++bil_state_ss) [bil_state_set_pc_def,
   bil_state_normalise_pc_execs]);
 
@@ -949,7 +949,7 @@ val bil_exec_step_execs = store_thm ("bil_exec_step_execs",
 ``!p st. bil_is_valid_state p st ==>
          (if bil_state_is_terminated st then
            (bil_exec_step p st = st)
-         else ((bil_exec_step p st).execs = SUC (st.execs)))``,
+         else ((bil_exec_step p st).bst_execs = SUC (st.bst_execs)))``,
 
 
 REPEAT STRIP_TAC >>
@@ -969,7 +969,7 @@ Cases_on `stmt` >> (
 
 val bil_state_EQ_EXCEPT_EXECS_def = Define `
   bil_state_EQ_EXCEPT_EXECS st st' <=>
-  ((st' with execs := 0) = (st with execs := 0))`;
+  ((st' with bst_execs := 0) = (st with bst_execs := 0))`;
 
 val bil_state_EQ_EXCEPT_EXECS_ALT_DEF = save_thm ("bil_state_EQ_EXCEPT_EXECS_ALT_DEF",
 SIMP_RULE (std_ss++bil_state_ss) [DB.fetch "-" "bil_state_t_component_equality"]
@@ -1021,7 +1021,7 @@ SIMP_TAC std_ss [Once bil_state_EQ_EXCEPT_EXECS_ALT_DEF] >>
 REPEAT GEN_TAC >> STRIP_TAC >>
 Cases >> ASM_SIMP_TAC std_ss [bil_exec_stmt_def] >| [
   ASM_SIMP_TAC std_ss [bil_exec_stmt_declare_def, LET_DEF] >>
-  Q.HO_MATCH_ABBREV_TAC `bil_state_EQ_EXCEPT_EXECS (if (is_env_regular env) then _ else _) _` >>
+  Q.HO_MATCH_ABBREV_TAC `bil_state_EQ_EXCEPT_EXECS (if (bil_is_regular_env env) then _ else _) _` >>
   CASE_TAC >- (
     MATCH_MP_TAC bil_state_incr_pc_CHANGE_EXECS >>
     ASM_SIMP_TAC (std_ss++bil_state_ss) [bil_state_EQ_EXCEPT_EXECS_ALT_DEF]
@@ -1030,7 +1030,7 @@ Cases >> ASM_SIMP_TAC std_ss [bil_exec_stmt_def] >| [
 
 
   ASM_SIMP_TAC std_ss [bil_exec_stmt_assign_def, LET_DEF] >>
-  Q.HO_MATCH_ABBREV_TAC `bil_state_EQ_EXCEPT_EXECS (if (is_env_regular env) then _ else _) _` >>
+  Q.HO_MATCH_ABBREV_TAC `bil_state_EQ_EXCEPT_EXECS (if (bil_is_regular_env env) then _ else _) _` >>
   CASE_TAC >- (
     MATCH_MP_TAC bil_state_incr_pc_CHANGE_EXECS >>
     ASM_SIMP_TAC (std_ss++bil_state_ss) [bil_state_EQ_EXCEPT_EXECS_ALT_DEF]
@@ -1093,7 +1093,7 @@ REPEAT STRIP_TAC >>
 Cases_on `bil_state_is_terminated st2` >- (
   ASM_SIMP_TAC std_ss [bil_state_EQ_EXCEPT_EXECS_ALT_DEF]
 ) >>
-Cases_on `bil_get_current_statement p st1.pc` >- (
+Cases_on `bil_get_current_statement p st1.bst_pc` >- (
   ASM_SIMP_TAC (std_ss++bil_state_ss) [bil_state_EQ_EXCEPT_EXECS_ALT_DEF,
     bil_state_set_failed_def]
 ) >>
@@ -1274,7 +1274,7 @@ val bil_exec_step_FUNPOW_EXECS_ADD = store_thm ("bil_exec_step_FUNPOW_EXECS_ADD"
 ``!p state n.
     bil_is_valid_state p state ==> bil_is_valid_program p ==>
     (!i. i < n ==> ~(bil_state_is_terminated (FUNPOW (bil_exec_step p) i state))) ==>
-    ((FUNPOW (bil_exec_step p) n state).execs = state.execs + n)``,
+    ((FUNPOW (bil_exec_step p) n state).bst_execs = state.bst_execs + n)``,
 
 GEN_TAC >> GEN_TAC >>
 Induct_on `n` >- (
@@ -1295,7 +1295,7 @@ val bil_exec_steps_opt_EXECS_ADD = store_thm ("bil_exec_steps_opt_EXECS_ADD",
     bil_is_valid_state p state ==> bil_is_valid_program p ==>
     (case mo of NONE => T | SOME m => b <= m) ==>
     (bil_exec_steps_opt p state b mo = SOME (c, state')) ==>
-    (state'.execs = state.execs + (c - b))``,
+    (state'.bst_execs = state.bst_execs + (c - b))``,
 
 SIMP_TAC std_ss [bil_exec_steps_opt_EQ_SOME] >>
 REPEAT STRIP_TAC >>
@@ -1308,7 +1308,7 @@ val bil_exec_step_n_EXECS_ADD = store_thm ("bil_exec_step_n_EXECS_ADD",
 ``!p state state' n c.
     bil_is_valid_state p state ==> bil_is_valid_program p ==>
     (bil_exec_step_n p state n = (c, state')) ==>
-    (state'.execs = state.execs + c)``,
+    (state'.bst_execs = state.bst_execs + c)``,
 
 REPEAT STRIP_TAC >>
 FULL_SIMP_TAC std_ss [bil_exec_step_n_EQ_THM] >>
@@ -1321,7 +1321,7 @@ val bil_exec_steps_EXECS_ADD = store_thm ("bil_exec_steps_EXECS_ADD",
 ``!p state state' c.
     bil_is_valid_state p state ==> bil_is_valid_program p ==>
     (bil_exec_steps p state = SOME (c, state')) ==>
-    (state'.execs = state.execs + c)``,
+    (state'.bst_execs = state.bst_execs + c)``,
 
 REPEAT STRIP_TAC >>
 MP_TAC (Q.SPECL [`p`, `state`, `state'`, `0`, `NONE`] bil_exec_steps_opt_EXECS_ADD) >>
@@ -1336,28 +1336,28 @@ FULL_SIMP_TAC std_ss [bil_exec_steps_def]);
 
 
 val bil_state_set_failed_SAME_ENV = store_thm ("bil_state_set_failed_SAME_ENV",
-  ``!st msg. (bil_state_set_failed st msg).environ = st.environ``,
+  ``!st msg. (bil_state_set_failed st msg).bst_environ = st.bst_environ``,
 SIMP_TAC (std_ss++bil_state_ss) [bil_state_set_failed_def]);
 
 
 val bil_state_normalise_pc_SAME_ENV = store_thm ("bil_state_normalise_pc_SAME_ENV",
-  ``!p st. (bil_state_normalise_pc p st).environ = st.environ``,
+  ``!p st. (bil_state_normalise_pc p st).bst_environ = st.bst_environ``,
 REPEAT STRIP_TAC >>
 SIMP_TAC std_ss [bil_state_normalise_pc_def] >>
 CASE_TAC >> SIMP_TAC (std_ss++bil_state_ss) []);
 
 
 val bil_state_incr_pc_SAME_ENV = store_thm ("bil_state_incr_pc_SAME_ENV",
-  ``!p st. (bil_state_incr_pc p st).environ = st.environ``,
+  ``!p st. (bil_state_incr_pc p st).bst_environ = st.bst_environ``,
 SIMP_TAC (std_ss++bil_state_ss) [bil_state_incr_pc_def, bil_state_normalise_pc_SAME_ENV]);
 
 val bil_state_set_pc_SAME_ENV = store_thm ("bil_state_set_pc_SAME_ENV",
-  ``!p st l. (bil_state_set_pc p st l).environ = st.environ``,
+  ``!p st l. (bil_state_set_pc p st l).bst_environ = st.bst_environ``,
 SIMP_TAC (std_ss++bil_state_ss) [bil_state_set_pc_def, bil_state_normalise_pc_SAME_ENV]);
 
 
 val bil_exec_stmt_jmp_SAME_ENV = store_thm("bil_exec_stmt_jmp_SAME_ENV",
-  ``!p st l. (bil_exec_stmt_jmp p l st).environ = st.environ``,
+  ``!p st l. (bil_exec_stmt_jmp p l st).bst_environ = st.bst_environ``,
 SIMP_TAC std_ss [bil_exec_stmt_jmp_def] >>
 REPEAT STRIP_TAC >>
 COND_CASES_TAC >> SIMP_TAC (std_ss++bil_state_ss) [bil_state_set_pc_SAME_ENV]);
@@ -1365,7 +1365,7 @@ COND_CASES_TAC >> SIMP_TAC (std_ss++bil_state_ss) [bil_state_set_pc_SAME_ENV]);
 
 
 val bil_exec_stmt_cjmp_SAME_ENV = store_thm("bil_exec_stmt_cjmp_SAME_ENV",
-  ``!p e st l1 l2. (bil_exec_stmt_cjmp p e l1 l2 st).environ = st.environ``,
+  ``!p e st l1 l2. (bil_exec_stmt_cjmp p e l1 l2 st).bst_environ = st.bst_environ``,
 SIMP_TAC std_ss [bil_exec_stmt_cjmp_def] >>
 REPEAT STRIP_TAC >>
 REPEAT CASE_TAC >> SIMP_TAC (std_ss++bil_state_ss) [bil_exec_stmt_jmp_SAME_ENV,
@@ -1374,12 +1374,12 @@ REPEAT CASE_TAC >> SIMP_TAC (std_ss++bil_state_ss) [bil_exec_stmt_jmp_SAME_ENV,
 
 
 val bil_exec_stmt_halt_SAME_ENV = store_thm("bil_exec_stmt_halt_SAME_ENV",
-  ``!e st. (bil_exec_stmt_halt e st).environ = st.environ``,
+  ``!e st. (bil_exec_stmt_halt e st).bst_environ = st.bst_environ``,
 SIMP_TAC (std_ss++bil_state_ss) [bil_exec_stmt_halt_def]);
 
 
 val bil_exec_stmt_assert_SAME_ENV = store_thm("bil_exec_stmt_assert_SAME_ENV",
-  ``!p e st. (bil_exec_stmt_assert p e st).environ = st.environ``,
+  ``!p e st. (bil_exec_stmt_assert p e st).bst_environ = st.bst_environ``,
 SIMP_TAC (std_ss++bil_state_ss) [bil_exec_stmt_assert_def] >>
 REPEAT STRIP_TAC >>
 REPEAT CASE_TAC >> SIMP_TAC (std_ss++bil_state_ss) [bil_state_incr_pc_SAME_ENV,
@@ -1388,7 +1388,7 @@ REPEAT CASE_TAC >> SIMP_TAC (std_ss++bil_state_ss) [bil_state_incr_pc_SAME_ENV,
 
 
 val bil_exec_stmt_assume_SAME_ENV = store_thm("bil_exec_stmt_assume_SAME_ENV",
-  ``!p e st. (bil_exec_stmt_assume p e st).environ = st.environ``,
+  ``!p e st. (bil_exec_stmt_assume p e st).bst_environ = st.bst_environ``,
 SIMP_TAC (std_ss++bil_state_ss) [bil_exec_stmt_assume_def] >>
 REPEAT STRIP_TAC >>
 REPEAT CASE_TAC >> SIMP_TAC (std_ss++bil_state_ss) [bil_state_incr_pc_SAME_ENV,
@@ -1397,28 +1397,28 @@ REPEAT CASE_TAC >> SIMP_TAC (std_ss++bil_state_ss) [bil_state_incr_pc_SAME_ENV,
 
 
 val bil_exec_stmt_declare_ENV = store_thm("bil_exec_stmt_declare_ENV",
-  ``!p vn vty st. (bil_exec_stmt_declare p vn vty st).environ =
-      if (bil_env_varname_is_bound st.environ vn) then st.environ else
+  ``!p vn vty st. (bil_exec_stmt_declare p vn vty st).bst_environ =
+      if (bil_env_varname_is_bound st.bst_environ vn) then st.bst_environ else
       (bil_env_update vn (bil_declare_initial_value vty) vty
-            st.environ)``,
+            st.bst_environ)``,
 
 SIMP_TAC (std_ss++bil_state_ss) [bil_exec_stmt_declare_def, LET_DEF] >>
 REPEAT STRIP_TAC >>
 REPEAT CASE_TAC >> (
    FULL_SIMP_TAC (std_ss++bil_state_ss) [bil_state_incr_pc_SAME_ENV,
-     bil_state_set_failed_SAME_ENV, is_env_regular_def]
+     bil_state_set_failed_SAME_ENV, bil_is_regular_env_def]
 ) >>
-Cases_on `st.environ` >> FULL_SIMP_TAC std_ss [bil_env_update_def] >>
+Cases_on `st.bst_environ` >> FULL_SIMP_TAC std_ss [bil_env_update_def] >>
 Cases_on `vty` >> FULL_SIMP_TAC std_ss [bil_declare_initial_value_def,
-  is_env_regular_def, type_of_bil_val_def]);
+  bil_is_regular_env_def, type_of_bil_val_def]);
 
 
 val bil_exec_stmt_assign_ENV = store_thm("bil_exec_stmt_assign_ENV",
   ``!p v e st.
-      (bil_exec_stmt_assign p v e st).environ =
-      (if is_env_regular (bil_env_write v (bil_eval_exp e st.environ) st.environ) then
-         (bil_env_write v (bil_eval_exp e st.environ) st.environ)
-       else st.environ)``,
+      (bil_exec_stmt_assign p v e st).bst_environ =
+      (if bil_is_regular_env (bil_env_write v (bil_eval_exp e st.bst_environ) st.bst_environ) then
+         (bil_env_write v (bil_eval_exp e st.bst_environ) st.bst_environ)
+       else st.bst_environ)``,
 
 SIMP_TAC (std_ss++bil_state_ss) [bil_exec_stmt_assign_def, LET_DEF] >>
 REPEAT STRIP_TAC >>
@@ -1429,7 +1429,7 @@ REPEAT CASE_TAC >> (
 
 
 val bil_exec_stmt_ENV_ORDER = store_thm ("bil_exec_stmt_ENV_ORDER",
-``!p st stmt. bil_env_order st.environ (bil_exec_stmt p stmt st).environ``,
+``!p st stmt. bil_env_order st.bst_environ (bil_exec_stmt p stmt st).bst_environ``,
 
 Cases_on `stmt` >> (
   SIMP_TAC (std_ss++boolSimps.LIFT_COND_ss) [bil_exec_stmt_def, bil_exec_stmt_jmp_SAME_ENV,
@@ -1439,7 +1439,7 @@ Cases_on `stmt` >> (
 ) >- (
   REPEAT STRIP_TAC >>
   rename1 `bil_var_name v` >>
-  Cases_on `bil_env_varname_is_bound st.environ (bil_var_name v)` >> ASM_REWRITE_TAC[] >>
+  Cases_on `bil_env_varname_is_bound st.bst_environ (bil_var_name v)` >> ASM_REWRITE_TAC[] >>
   MATCH_MP_TAC bil_env_order_update >>
   ASM_REWRITE_TAC[] >>
   Cases_on `bil_var_type v` >> (
@@ -1453,7 +1453,7 @@ Cases_on `stmt` >> (
 
 
 val bil_exec_step_ENV_ORDER = store_thm ("bil_exec_step_ENV_ORDER",
-``!p st. bil_env_order st.environ (bil_exec_step p st).environ``,
+``!p st. bil_env_order st.bst_environ (bil_exec_step p st).bst_environ``,
 
 REPEAT GEN_TAC >>
 SIMP_TAC std_ss [bil_exec_step_def] >>
@@ -1465,7 +1465,7 @@ REPEAT CASE_TAC >> (
 
 
 val bil_exec_step_FUNPOW_ENV_ORDER = store_thm ("bil_exec_step_FUNPOW_ENV_ORDER",
-``!p n st. bil_env_order st.environ (FUNPOW (bil_exec_step p) n st).environ``,
+``!p n st. bil_env_order st.bst_environ (FUNPOW (bil_exec_step p) n st).bst_environ``,
 
 GEN_TAC >>
 Induct >> (
@@ -1473,21 +1473,21 @@ Induct >> (
 ) >>
 GEN_TAC >>
 MATCH_MP_TAC (SIMP_RULE std_ss [AND_IMP_INTRO] bil_env_order_TRANS) >>
-Q.EXISTS_TAC `(bil_exec_step p st).environ` >>
+Q.EXISTS_TAC `(bil_exec_step p st).bst_environ` >>
 ASM_SIMP_TAC std_ss [bil_exec_step_ENV_ORDER]);
 
 
 
 val bil_exec_steps_ENV_ORDER = store_thm ("bil_exec_steps_ENV_ORDER",
 ``!p c st st'. (bil_exec_steps p st = SOME (c, st')) ==>
-  bil_env_order st.environ st'.environ``,
+  bil_env_order st.bst_environ st'.bst_environ``,
 
 SIMP_TAC std_ss [bil_exec_steps_EQ_SOME, bil_exec_step_FUNPOW_ENV_ORDER]);
 
 
 val bil_exec_step_n_ENV_ORDER = store_thm ("bil_exec_step_n_ENV_ORDER",
 ``!p c n st st'. (bil_exec_step_n p st n = (c, st')) ==>
-  bil_env_order st.environ st'.environ``,
+  bil_env_order st.bst_environ st'.bst_environ``,
 
 SIMP_TAC std_ss [bil_exec_step_n_EQ_THM, bil_exec_step_FUNPOW_ENV_ORDER]);
 
